Added comments

deds.v
@@ -1,36 +1,57 @@
+(* 
+ * Classical logic is required for decision-making on 
+ * labeling and sub-formulas. Classical logic is not
+ * mandatory for the theories formalized in this proof,
+ * but help us avoid dragging too much information with
+ * us in the K-structures.
+ *)
 Axiom classic : forall (P : Prop), P \/ ~ P.
 
+(* Assume the event-set E and property-set P as parameters to this theory *)
 Parameter E P : Set.
+
+(* Define the characteristic function for uncontrollable events *)
 Parameter U : E -> Prop.
 
+(* 
+ * Define the K-structure inductively as a four-tuple
+ * for state-space X, labeling function (having the
+ * X -> P -> Prop signature), transition relation
+ * (having the X -> E -> X -> Prop signature) and
+ * initial state.
+ *)
 Inductive K : Type := klts : forall (X : Set),
   (X -> P -> Prop) -> (X -> E -> X -> Prop) -> X -> K.
 
+(* Define the reflexive-transitive closure of a transition relation *)
 Inductive trans (X : Set) (step : X -> E -> X -> Prop) : X -> X -> Prop :=
   | trans_refl : forall (x : X), trans X step x x
-  | trans_closed : forall (x y x' : X) (e : E), step x e y ->
-    trans X step y x' -> trans X step x x'.
+  | trans_closed : forall (x y x' : X) (e : E), 
+    trans X step y x' -> step x e y -> trans X step x x'.
 
+(* Define partial bisimulation *)
 Definition pbis (k' k : K) : Prop :=
   match (k', k) with
   | (klts X' L' step' x', klts X L step x) =>
-      exists R : X' -> X -> Prop, R x' x /\
-        forall (y' : X') (y : X), R y' y ->
-          (forall (p : P), L' y' p <-> L y p) /\
-          (forall (e : E) (z' : X'), step' y' e z' ->
-            exists z : X, step y e z /\ R z' z) /\
-          (forall (e : E) (z : X), U e -> step y e z ->
-            exists z' : X', step' y' e z' /\ R z' z)
+    exists R : X' -> X -> Prop, R x' x /\
+    forall (y' : X') (y : X), R y' y ->
+      (forall (p : P), L' y' p <-> L y p) /\
+      (forall (e : E) (z' : X'), step' y' e z' ->
+        exists z : X, step y e z /\ R z' z) /\
+      (forall (e : E) (z : X), U e -> step y e z ->
+        exists z' : X', step' y' e z' /\ R z' z)
   end.
 
+(* Define the set of B-formulas *)
 Inductive B : Set :=
   | true : B
   | false : B
   | prop : P -> B
-  | neg : B -> B
   | and : B -> B -> B
-  | or : B -> B -> B.
+  | or : B -> B -> B
+  | neg : B -> B.
 
+(* Define the set of F-formulas *)
 Inductive F : Set :=
   | basic : B -> F
   | conj : F -> F -> F
@@ -42,6 +63,11 @@ Inductive F : Set :=
   | can : E -> F
   | dlf : F.
 
+(* 
+ * We need an additional well-formedness test to assure
+ * that formulas of type <e>f are restricted in such a
+ * way that e is controllable.
+ *)
 Fixpoint wf (f : F) : Prop :=
   match f with
   | conj f g => wf f /\ wf g
@@ -52,105 +78,142 @@ Fixpoint wf (f : F) : Prop :=
   | _ => True
   end.
 
+(* Define validity for B-formulas w.r.t a K-structure *)
 Fixpoint bval (X : Set) (L : X -> P -> Prop) (x : X) (b : B) : Prop :=
   match b with
   | true => True
   | false => False
   | prop p => L x p
-  | neg b => ~ bval X L x b
   | and b c => bval X L x b /\ bval X L x c
   | or b c => bval X L x b \/ bval X L x c
+  | neg b => ~ bval X L x b
   end.
 
-Fixpoint val (k : K) (f : F) : Prop :=
+(* Define validity for F-formulas w.r.t a K-structure *)
+Fixpoint fval (k : K) (f : F) : Prop := 
   match (k, f) with
   | (klts X L step x, basic b) => bval X L x b
-  | (_, conj f g) => val k f /\ val k g
-  | (klts X L step x, disj b f) => bval X L x b \/ val k f
+  | (klts X L step x, conj f g) => fval k f /\ fval k g
+  | (klts X L step x, disj b f) => bval X L x b \/ fval k f
   | (klts X L step x, all e f) => forall (x' : X),
-    step x e x' -> val (klts X L step x') f
+    step x e x' -> fval (klts X L step x') f
   | (klts X L step x, ex e f) => exists x' : X,
-    step x e x' /\ val (klts X L step x') f
+    step x e x' /\ fval (klts X L step x') f
   | (klts X L step x, box f) => forall (x' : X),
-    trans X step x x' -> val (klts X L step x') f
+    trans X step x x' -> fval (klts X L step x') f
   | (klts X L step x, diam b) => exists x' : X,
     trans X step x x' /\ bval X L x' b
   | (klts X L step x, can e) => exists x' : X, step x e x'
-  | (klts X L step x, dlf) => exists e : E, exists x' : X, step x e x'
+  | (klts X L step x, dlf) => exists e : E, 
+    exists x' : X, step x e x'
   end.
 
-Inductive red (X : Set) (L : X -> P -> Prop) (x : X) : F -> E -> F -> Prop :=
-  | red_basic : forall (b : B) (e : E), red X L x (basic b) e (basic true)
-  | red_and : forall (f g f' g' : F) (e : E), red X L x f e f' ->
-    red X L x g e g' -> red X L x (conj f g) e (conj f' g')
-  | red_or_left : forall (f : F) (b : B) (e : E), 
-    bval X L x b -> red X L x (disj b f) e (basic true)
-  | red_or_right : forall (f f' : F) (b : B) (e : E),
-    ~ bval X L x b -> red X L x f e f' -> red X L x (disj b f) e f'
-  | red_all_pos : forall (f : F) (e : E), red X L x (all e f) e f
-  | red_all_neg : forall (f : F) (e e' : E), e <> e' -> red X L x (all e f) e' (basic true)
-  | red_ex_pos : forall (f : F) (e : E), red X L x (ex e f) e f
-  | red_ex_neg : forall (f : F) (e e' : E), red X L x (ex e f) e' (basic true)
-  | red_box : forall (f f' : F) (e : E), red X L x f e f' ->
-    red X L x (box f) e (conj (box f) f')
-  | red_diam : forall (b : B) (e : E), red X L x (diam b) e (basic true)
-  | red_can : forall (e e' : E), red X L x (can e) e' (basic true)
-  | red_dlf : forall (e : E), red X L x dlf e (basic true).
-
+(* Define sub-formulas as an inductive predicate *)
 Inductive sub (X : Set) (L : X -> P -> Prop) (x : X) : F -> F -> Prop :=
   | sub_refl : forall (f : F), sub X L x f f
-  | sub_and_left : forall (f g h : F), sub X L x f g -> sub X L x f (conj g h)
-  | sub_and_right : forall (f g h : F), sub X L x f h -> sub X L x f (conj g h)
-  | sub_or : forall (f g : F) (b : B), ~ bval X L x b -> 
-    sub X L x f g -> sub X L x f (disj b g)
+  | sub_conj_left : forall (f g h : F), sub X L x f g -> sub X L x f (conj g h)
+  | sub_conj_right : forall (f g h : F), sub X L x f h -> sub X L x f (conj g h)
+  | sub_disj : forall (f g : F) (b : B), ~ bval X L x b -> sub X L x f g -> sub X L x f (disj b g)
   | sub_box : forall (f g : F), sub X L x f g -> sub X L x f (box g).
 
+(* Define the unfolded initial transition relation -->0 *)
+Inductive zero (X : Set) (L : X -> P -> Prop) 
+    (step : X -> E -> X -> Prop) : X * F -> E -> X * F -> Prop :=
+  | zero_basic : forall (x x' : X) (e : E) (b : B), 
+    step x e x' -> zero X L step (x, basic b) e (x', basic true)
+  | zero_conj_incl : forall (x x' : X) (e : E) (f g f' g' : F),
+    zero X L step (x, f) e (x', f') -> zero X L step (x, g) e (x', g') ->
+    sub X L x' g' f' -> zero X L step (x, conj f g) e (x', f')
+  | zero_conj_excl : forall (x x' : X) (e : E) (f g f' g' : F),
+    zero X L step (x, f) e (x', f') -> zero X L step (x, g) e (x', g') ->
+    ~ sub X L x' g' f' -> zero X L step (x, conj f g) e (x', conj f' g')
+  | zero_disj_left : forall (x x' : X) (e : E) (b : B) (f : F),
+    bval X L x b -> step x e x' -> zero X L step (x, disj b f) e (x', basic true)
+  | zero_disj_right : forall (x x' : X) (e : E) (b : B) (f f' : F),
+    ~ bval X L x b -> zero X L step (x, f) e (x', f') ->
+    zero X L step (x, disj b f) e (x', f')
+  | zero_all_pos : forall (x x' : X) (e : E) (f : F),
+    step x e x' -> zero X L step (x, all e f) e (x', f)
+  | zero_all_neg : forall (x x' : X) (e e' : E) (f : F), e <> e' ->
+    step x e' x' -> zero X L step (x, all e f) e' (x', basic true)
+  | zero_ex_pos : forall (x x' : X) (e : E) (f : F),
+    step x e x' -> zero X L step (x, ex e f) e (x', f)
+  | zero_ex_neg : forall (x x' : X) (e e' : E) (f : F),
+    step x e' x' -> zero X L step (x, ex e f) e' (x', basic true)
+  | zero_box_incl : forall (x x' : X) (e : E) (f f' : F),
+    zero X L step (x, f) e (x', f') -> sub X L x' f' f ->
+    zero X L step (x, box f) e (x', box f)
+  | zero_box_excl : forall (x x' : X) (e : E) (f f' : F),
+    zero X L step (x, f) e (x', f') -> ~ sub X L x' f' f ->
+    zero X L step (x, box f) e (x', conj (box f) f')
+  | zero_diam : forall (x x' : X) (e : E) (b : B),
+    step x e x' -> zero X L step (x, diam b) e (x', basic true)
+  | zero_can : forall (x x' : X) (e e' : E), step x e' x' ->
+    zero X L step (x, can e) e' (x', basic true)
+  | zero_dlf : forall (x x' : X) (e : E), step x e x' ->
+    zero X L step (x, dlf) e (x', basic true).
+
+(* 
+ * Define the synthesizability predicate by means of an
+ * inductive predicate to closely resemble the derivation
+ * rules proposed in the paper.
+ *)
 Inductive syn (X : Set) (L : X -> P -> Prop)
-    (step : X * F -> E -> X * F -> Prop) : X * F -> F -> Prop :=
-  | syn_basic : forall (x : X) (b : B) (g : F), bval X L x b -> syn X L step (x, g) (basic b)
-  | syn_and : forall (x : X) (f1 f2 g : F), syn X L step (x, g) f1 ->
+  (step : X * F -> E -> X * F -> Prop) : X * F -> F -> Prop :=
+  | syn_basic : forall (x : X) (g : F) (b : B), bval X L x b -> syn X L step (x, g) (basic b)
+  | syn_conj : forall (x : X) (g f1 f2 : F), syn X L step (x, g) f1 ->
     syn X L step (x, g) f2 -> syn X L step (x, g) (conj f1 f2)
-  | syn_or_left : forall (x : X) (b : B) (f g : F),
-    bval X L x b -> syn X L step (x, g) (disj b f)
-  | syn_or_right : forall (x : X) (b : B) (f g : F),
-    syn X L step (x, g) f -> syn X L step (x, g) (disj b f)
-  | syn_all : forall (x : X) (f g : F) (e : E), syn X L step (x, g) (all e f)
-  | syn_ex : forall (x x' : X) (f g g' : F) (e : E),
-    step (x, g) e (x', g') -> sub X L x' f g' ->
-    syn X L step (x', g') f -> syn X L step (x, g) (ex e f)
-  | syn_box : forall (x : X) (f g : F), syn X L step (x, g) f -> 
-    syn X L step (x, g) (box f)
-  | syn_diam : forall (x x' : X) (b : B) (g g' : F),
-    trans (X * F) step (x, g) (x', g') -> bval X L x' b ->
-    syn X L step (x, g) (diam b)
-  | syn_can : forall (x x' : X) (g g' : F) (e : E),
+  | syn_disj_left : forall (x : X) (g f : F) (b : B), bval X L x b -> syn X L step (x, g) (disj b f)
+  | syn_disj_right : forall (x : X) (g f : F) (b : B), syn X L step (x, g) f -> 
+    syn X L step (x, g) (disj b f)
+  | syn_all : forall (x : X) (e : E) (g f : F), syn X L step (x, g) (all e f)
+  | syn_ex : forall (x x' : X) (e : E) (g g' f : F), step (x, g) e (x', g') -> 
+    sub X L x' f g' -> syn X L step (x', g') f -> syn X L step (x, g) (ex e f)
+  | syn_box : forall (x : X) (g f : F), syn X L step (x, g) f -> syn X L step (x, g) (box f)
+  | syn_diam : forall (x x' : X) (g g' : F) (b : B), bval X L x' b ->
+    trans (X * F) step (x, g) (x', g') -> syn X L step (x, g) (diam b)
+  | syn_can : forall (x x' : X) (e : E) (g g' : F),
     step (x, g) e (x', g') -> syn X L step (x, g) (can e)
-  | syn_dlf : forall (x x' : X) (g g' : F) (e : E),
+  | syn_dlf : forall (x x' : X) (e : E) (g g' : F),
     step (x, g) e (x', g') -> syn X L step (x, g) dlf.
 
+(* Restrict a transition relation to only uncontrollable steps *)
 Definition unctrl (X : Set) (step : X -> E -> X -> Prop) (x : X) (e : E) (x' : X) : Prop :=
   step x e x' /\ U e.
 
+(* 
+ * Give the fixpoint definition for the iterative steps
+ * in constructing the transition relation for the synthesis
+ * result. The first step, where n = 0, is directly equal
+ * to the -->0 relation defined previously. For the
+ * n+1 case, we restrict the -->n relation in such a
+ * way that only the steps (x, f) -(e)->n (x', f') such
+ * that for all (x', f') -(s)->*n (x'', f'') and s taken
+ * from U* and syn (x'', f'') f'' are inherited.
+ *)
 Fixpoint rel (n : nat) (X : Set) (L : X -> P -> Prop)
   (step : X -> E -> X -> Prop) (xf : X * F) (e : E) (xf' : X * F) : Prop :=
   match n with
-  | 0 => step (fst xf) e (fst xf') /\ red X L (fst xf) (snd xf) e (snd xf')
-  | S n => rel n X L step xf e xf' /\ (U e \/
-    forall (xf'' : X * F), trans (X * F) (unctrl (X * F) (rel n X L step)) xf' xf'' -> 
+  | 0 => zero X L step xf e xf'
+  | S n => rel n X L step xf e xf' /\ (U e \/ forall (xf'' : X * F),
+    trans (X * F) (unctrl (X * F) (rel n X L step)) xf' xf'' ->
     syn X L (rel n X L step) xf'' (snd xf''))
   end.
 
+(* Define n-th iteration of the synthesis result *)
 Definition S (k : K) (f : F) (n : nat) : K :=
-  match k with
-  | klts X L step x => 
-    klts (X * F) (fun xf => L (fst xf)) (rel n X L step) (x, f)
+  match k with 
+  | klts X L step x => klts (X * F) (fun xf => L (fst xf))
+      (rel n X L step) (x, f)
   end.
 
+(* Define a predicate to check whether synthesis is finished *)
 Definition complete (n : nat) (X : Set) (L : X -> P -> Prop)
-  (step : X -> E -> X -> Prop) (x : X) (f : F) : Prop :=
-    forall (x' : X) (f' : F), trans (X * F) (rel n X L step) (x, f) (x', f') ->
-      syn X L (rel n X L step) (x', f') f'.
+  (step : X -> E -> X -> Prop) (xf : X * F) : Prop :=
+  forall (xf' : X * F), trans (X * F) (rel n X L step) xf xf' ->
+  syn X L (rel n X L step) xf' (snd xf').
 
+(* If x -->* y and y -->* z then x -->* z *)
 Lemma trans_cat : forall (X : Set) (step : X -> E -> X -> Prop) (x y z : X),
   trans X step x y -> trans X step y z -> trans X step x z.
 Proof.
@@ -158,135 +221,46 @@ Proof.
   apply trans_closed with y e ; auto.
 Qed.
 
-Lemma complete_impl_syn : forall (X : Set) (L : X -> P -> Prop)
-  (step : X -> E -> X -> Prop) (x : X) (f : F) (n : nat),
-  complete n X L step x f -> syn X L (rel n X L step) (x, f) f.
+(* If (x, f) -(e)->0 (x', f') then x -(e)-> x' *)
+Lemma zero_impl_step : forall (f f' : F) (X : Set) (L : X -> P -> Prop)
+  (step : X -> E -> X -> Prop) (x x' : X) (e : E),
+  zero X L step (x, f) e (x', f') -> step x e x'.
 Proof.
-  intros X L step x f n Hcomplete ; unfold complete in *.
-  apply Hcomplete ; apply trans_refl.
+  intro f ; induction f ; intros f' X L step x x' e' Hzero ;
+    solve [ inversion Hzero ; auto ] || auto.
+  inversion Hzero ; apply IHf1 in H4 ; auto.
+  inversion Hzero ; auto.
+  apply IHf in H6 ; auto.
+  inversion Hzero ; auto.
+  apply IHf in H3 ; auto.
+  apply IHf in H3 ; auto.
 Qed.
 
-Lemma bval_expand : forall (X : Set) (L : X -> P -> Prop) (x : X) (g : F) (b : B),
-  bval X L x b <-> bval (X * F) (fun xf => L (fst xf)) (x, g) b.
+(* If (x, f) -(e)->n (x', f') then (x, f) -(e)->0 (x', f') *)
+Lemma rel_impl_zero : forall (n : nat) (f f' : F) (X : Set) 
+  (L : X -> P -> Prop) (step : X -> E -> X -> Prop) (x x' : X) (e : E),
+  rel n X L step (x, f) e (x', f') -> zero X L step (x, f) e (x', f').
 Proof.
-  intros X L x g b ; induction b ; split ; intro H ;
-    solve [ simpl in * ; tauto ] || idtac.
+  intro n ; induction n ; intros f f' X L step x x' e Hrel.
+  simpl in Hrel ; auto.
+  simpl in Hrel ; destruct Hrel as [ Hrel _ ].
+  apply IHn in Hrel ; auto.
 Qed.
 
-Lemma rel_impl_step_red : forall (n : nat) (X : Set) (L : X -> P -> Prop)
-  (step : X -> E -> X -> Prop) (x x' : X) (e : E) (f f' : F),
-    rel n X L step (x, f) e (x', f') -> step x e x' /\ red X L x f e f'.
+(* Synthesizability is inherited over sub-formulas *)
+Lemma sub_syn : forall (X : Set) (L : X -> P -> Prop)
+  (step : X * F -> E -> X * F -> Prop) (x : X) (f g h : F),
+  sub X L x f g -> syn X L step (x, h) g -> syn X L step (x, h) f.
 Proof.
-  intro n ; induction n ; intros X L step x x' e f f' Hrel ;
-    simpl in * ; destruct Hrel ; auto.
+  intros X L step x f g h Hsub Hsyn ; induction Hsub ; 
+    solve [ auto ] || solve [ inversion Hsyn ; 
+    contradiction || auto ] || auto.
 Qed.
 
-Lemma sub_syn : forall (X : Set) (L : X -> P -> Prop) 
-  (step : X -> E -> X -> Prop) (x : X) (f g h : F) (n : nat),
-  sub X L x f g -> syn X L (rel n X L step) (x, h) g ->
-  syn X L (rel n X L step) (x, h) f.
-Proof.
-  intros X L step x f g h n Hsub Hsyn ; induction Hsub ; 
-    solve [ auto ] || solve [ inversion Hsyn ; auto ] || auto.
-  inversion Hsyn ; contradiction || auto.
-Qed.
-
-Lemma sub_and : forall (X : Set) (L : X -> P -> Prop) (x : X) (f g h : F),
-  sub X L x (conj f g) h -> sub X L x f h /\ sub X L x g h.
-Proof.
-  intros X L x f g h Hsub ; assert (exists i : F, i = conj f g) as H by eauto.
-  destruct H as [ i H ] ; rewrite <- H in *.
-  induction Hsub ; rewrite H in *.
-  split ; [ apply sub_and_left | apply sub_and_right ] ; apply sub_refl.
-  split ; apply sub_and_left ; tauto.
-  split ; apply sub_and_right ; tauto.
-  split ; apply sub_or ; tauto.
-  split ; apply sub_box ; tauto.
-Qed.
-
-Lemma sub_not_or : forall (X : Set) (L : X -> P -> Prop) (x : X) (b : B) (f g : F),
-  ~ bval X L x b -> sub X L x (disj b f) g -> sub X L x f g.
-Proof.
-  intros X L x b f g Hbval Hsub ; assert (exists h : F, h = disj b f) as H by eauto.
-  destruct H as [ i H ] ; rewrite <- H in *.
-  induction Hsub ; rewrite H in *.
-  apply sub_or ; apply sub_refl || auto.
-  apply sub_and_left ; auto.
-  apply sub_and_right ; auto.
-  apply sub_or ; auto.
-  apply sub_box ; auto.
-Qed.
-
-Lemma sub_all : forall (X : Set) (L : X -> P -> Prop) (x x' : X) (e : E) (f g g' : F),
-  sub X L x (all e f) g -> red X L x g e g' -> sub X L x' f g'.
-Proof.
-  intros X L x x' e f g g' Hsub Hred ; assert (exists h : F, h = all e f) as H by eauto.
-  destruct H as [ h H ] ; rewrite <- H in *.
-  revert Hred ; revert g' ; induction Hsub ; rewrite H in * ; intros g' Hred.
-  inversion Hred ; apply sub_refl || auto.
-  assert (e = e) by auto ; contradiction.
-  inversion Hred ; apply IHHsub in H2 ; apply sub_and_left || auto ; auto.
-  inversion Hred ; apply IHHsub in H5 ; apply sub_and_right || auto ; auto.
-  inversion Hred ; contradiction || auto.
-  inversion Hred ; apply IHHsub in H1 ; auto.
-  apply sub_and_right ; auto.
-Qed.
-
-Lemma sub_box_impl : forall (X : Set) (L : X -> P -> Prop) (x : X) 
-    (f g h : F), h = box f -> sub X L x h g -> sub X L x f g.
-Proof.
-  intros X L x f g h Heq Hsub ; induction Hsub ; rewrite Heq in *.
-  apply sub_box ; apply sub_refl ; auto.
-  apply sub_and_left ; auto.
-  apply sub_and_right ; auto.
-  apply sub_or ; auto.
-  apply sub_box ; auto.
-Qed.
-
-Lemma sub_box_trans : forall (n : nat) (X : Set)
-  (L : X -> P -> Prop) (step : X -> E -> X -> Prop)
-  (x x' : X) (f g g' : F), sub X L x (box f) g ->
-  trans (X * F) (rel n X L step) (x, g) (x', g') -> sub X L x' f g'.
-Proof.
-  assert (forall (X : Set) (L : X -> P -> Prop) (x x' : X)
-    (f g h : F) (e : E), h = box f -> sub X L x h g -> 
-    forall (g' : F), red X L x g e g' -> sub X L x' h g') as Hsub_red.
-  intros X L x x' f g h e Heq Hsub ; induction Hsub ;
-    rewrite Heq in * ; intros g' Hred.
-  inversion Hred ; apply sub_and_left ; apply sub_refl.
-  inversion Hred ; apply IHHsub in H1 ; apply sub_and_left || auto ; auto.
-  inversion Hred ; apply IHHsub in H4 ; apply sub_and_right || auto ; auto.
-  inversion Hred ; contradiction || auto.
-  inversion Hred ; apply IHHsub in H0 ; apply sub_and_right || auto ; auto.
-  assert (forall (X : Set) (L : X -> P -> Prop) (x : X) (f g h : F),
-    h = box f -> sub X L x h g -> sub X L x f g) as Hsub_box.
-  intros X L x f g h Heq Hsub ; induction Hsub ; rewrite Heq in *.
-  apply sub_box ; apply sub_refl ; auto.
-  apply sub_and_left ; auto.
-  apply sub_and_right ; auto.
-  apply sub_or ; auto.
-  apply sub_box ; auto.
-  intros n X L step x x' f g g' Hsub Htrans.
-  assert (exists xg : X * F, xg = (x, g)) as Hex by eauto.
-  assert (exists xg' : X * F, xg' = (x', g')) as Hex' by eauto.
-  destruct Hex as [ xg Heq ] ; rewrite <- Heq in *.
-  destruct Hex' as [ xg' Heq' ] ; rewrite <- Heq' in *.
-  revert Heq Hsub ; revert x g.
-  induction Htrans ; intros z g Heq Hsub ; rewrite Heq in *.
-  inversion Heq' ; replace x' with z in * by auto.
-  replace g' with g in * by auto.
-  apply Hsub_box with (f := f) in Hsub ; auto.
-  destruct y as [ y h ] ; apply rel_impl_step_red in H.
-  destruct H as [ _ Hred ].
-  assert ((y, h) = (y, h)) as H by auto.
-  apply IHHtrans in H ; auto.
-  apply Hsub_red with (x' := y) (f := f) (e := e) 
-    (g' := h) in Hsub ; auto.
-Qed.
-
+(* Validity is inherited over sub-formulas *)
 Lemma sub_val : forall (f g : F) (X : Set) (L : X -> P -> Prop)
   (step : X -> E -> X -> Prop) (x : X), sub X L x f g ->
-  val (klts X L step x) g -> val (klts X L step x) f.
+  fval (klts X L step x) g -> fval (klts X L step x) f.
 Proof.
   intros f g X L step x Hsub Hval ; induction Hsub ; auto.
   simpl in Hval ; destruct Hval ; auto.
@@ -295,679 +269,1096 @@ Proof.
   apply IHHsub ; apply Hval ; apply trans_refl.
 Qed.
 
-Theorem validity : forall (X : Set) (L : X -> P -> Prop)
-  (step : X -> E -> X -> Prop) (x : X) (f : F) (n : nat),
-  complete n X L step x f -> val (S (klts X L step x) f n) f.
+(* If f /\ g is a sub-formula of h then both f and g are sub-formulas of h *)
+Lemma sub_conj : forall (X : Set) (L : X -> P -> Prop) (x : X) (f g h : F),
+  sub X L x (conj f g) h -> sub X L x f h /\ sub X L x g h.
 Proof.
-  intros X L step x f n ; assert (sub X L x f f) as Hsub by apply sub_refl.
-  revert Hsub ; revert x ; generalize f at 2 3 4 as g.
-  induction f ; intros g x Hsub Hcomplete.
-  apply complete_impl_syn in Hcomplete.
-  apply sub_syn with (f := basic b) in Hcomplete ; auto.
-  inversion Hcomplete ; simpl ; apply bval_expand ; auto.
-  apply sub_and in Hsub ; destruct Hsub ; split ; auto.
-  destruct (classic (bval X L x b)) as [ H | H ].
-  simpl ; left ; apply bval_expand ; auto.
-  simpl ; right ; apply sub_not_or in Hsub ; apply IHf || auto ; auto.
-  simpl ; intros xg' Hstep ; destruct xg' as [ x' g' ] ; apply IHf ; auto.
-  apply rel_impl_step_red in Hstep ; destruct Hstep as [ _ Hred ].
-  apply sub_all with (x' := x') (g' := g') (f := f) in Hred ; auto.
-  intros x'' g'' Htrans ; apply Hcomplete ; apply trans_closed with (x', g') e ; auto.
-  assert (complete n X L step x g) as Hcomplete' by auto.
-  apply complete_impl_syn in Hcomplete.
-  apply sub_syn with (f := ex e f) in Hcomplete ; auto.
-  inversion Hcomplete ; exists (x', g') ; split ; solve [ auto ] || apply IHf ; auto.
-  intros x'' g'' Htrans ; apply Hcomplete' ; apply trans_closed with (x', g') e ; auto.  
-  simpl ; intros x' Htrans ; destruct x' as [ x' g' ].
-  apply IHf ; auto.
-  apply sub_box_trans with (f := f) in Htrans ; auto.
-  intros x'' g'' Htrans' ; apply Hcomplete.
-  apply trans_cat with (x', g') ; auto.
-  apply complete_impl_syn in Hcomplete.
-  apply sub_syn with (f := diam b) in Hcomplete ; auto.
-  inversion Hcomplete ; exists (x', g') ; split ; auto.
-  apply bval_expand ; auto.
-  apply complete_impl_syn in Hcomplete.
-  apply sub_syn with (f := can e) in Hcomplete ; auto.
-  inversion Hcomplete ; exists (x', g') ; auto.
-  apply complete_impl_syn in Hcomplete.
-  apply sub_syn with (f := dlf) in Hcomplete ; auto.
-  inversion Hcomplete ; exists e ; exists (x', g') ; auto.
+  intros X L x f g h Hsub.
+  assert (exists i : F, i = conj f g) as H by eauto.
+  destruct H as [ i Heq ] ; rewrite <- Heq in *.
+  revert Heq ; revert f g ; induction Hsub ; intros p q Heq ;
+    rewrite Heq in *.
+  split ; [ apply sub_conj_left | apply sub_conj_right ] ; apply sub_refl.
+  assert (conj p q = conj p q) as H by auto ; apply IHHsub in H.
+  split ; apply sub_conj_left ; tauto.
+  assert (conj p q = conj p q) as H by auto ; apply IHHsub in H.
+  split ; apply sub_conj_right ; tauto.
+  assert (conj p q = conj p q) as H' by auto ; apply IHHsub in H'.
+  split ; apply sub_disj ; tauto.
+  assert (conj p q = conj p q) as H by auto ; apply IHHsub in H.
+  split ; apply sub_box ; tauto.
 Qed.
 
-Lemma red_ex : forall (X : Set) (L : X -> P -> Prop) (x : X) (f : F) (e : E),
-  exists f' : F, red X L x f e f'.
+(* If b \/ f is a sub-formula of g and not x |= b then f \in sub (x, g) *)
+Lemma sub_disj_not : forall (X : Set) (L : X -> P -> Prop) (x : X) (b : B) (f g : F),
+  sub X L x (disj b f) g -> ~ bval X L x b -> sub X L x f g.
 Proof.
-  intros X L x f e ; induction f.
-  exists (basic true) ; apply red_basic.
-  destruct IHf1 as [ f1' Hred_f1 ].
-  destruct IHf2 as [ f2' Hred_f2 ].
-  exists (conj f1' f2') ; apply red_and ; auto.
+  intros X L x b f g Hsub Hbval.
+  assert (exists h : F, h = disj b f) as H by eauto.
+  destruct H as [ h Heq ] ; rewrite <- Heq in *.
+  revert Heq ; revert Hbval ; revert b f ; induction Hsub ; 
+    intros c f' Hbval Heq ; rewrite Heq in *.
+  apply sub_disj ; apply sub_refl || auto ; auto.
+  assert (disj c f' = disj c f') as H by auto.
+  apply IHHsub in H ; auto.
+  apply sub_conj_left ; auto.
+  assert (disj c f' = disj c f') as H by auto.
+  apply IHHsub in H ; auto.
+  apply sub_conj_right ; auto.
+  assert (disj c f' = disj c f') as H' by auto.
+  apply IHHsub in H' ; auto.
+  apply sub_disj ; auto.
+  assert (disj c f' = disj c f') as H' by auto.
+  apply IHHsub in H' ; auto.
+  apply sub_box ; auto.
+Qed.
+
+(* If []f \in sub (x, g) then f \in sub (x, g) *)
+Lemma sub_box_in : forall (X : Set) (L : X -> P -> Prop) 
+  (x : X) (f g : F), sub X L x (box f) g -> sub X L x f g.
+Proof.
+  intros X L x f g Hsub ; assert (exists h : F, h = box f) as H by eauto.
+  destruct H as [ h Heq ] ; rewrite <- Heq in *.
+  revert Heq ; revert f ; induction Hsub ;
+    intros f' Heq ; rewrite Heq in *.
+  apply sub_box ; apply sub_refl.
+  apply sub_conj_left ; apply IHHsub ; auto.
+  apply sub_conj_right ; apply IHHsub ; auto.
+  apply sub_disj ; auto.
+  apply sub_box ; auto.
+Qed.
+
+(* Prove transitivity of the sub-formula relation *)
+Lemma sub_trans : forall (X : Set) (L : X -> P -> Prop) (x : X) (f g h : F),
+  sub X L x f g -> sub X L x g h -> sub X L x f h.
+Proof.
+  intros X L x f g h Hsub Hsub' ; induction Hsub ; auto.
+  apply sub_conj in Hsub' ; destruct Hsub' ; auto.
+  apply sub_conj in Hsub' ; destruct Hsub' ; auto.
+  apply sub_disj_not in Hsub' ; auto.
+  apply sub_box_in in Hsub' ; auto.
+Qed.
+
+(* If (x, g) -(e)->0 (x', g') and [e]f \in sub (x, g) then f \in sub (x', g') *)
+Lemma sub_all : forall (f g g' : F) (X : Set) (L : X -> P -> Prop) 
+  (step : X -> E -> X -> Prop) (x y : X) (e : E), sub X L x (all e f) g -> 
+  zero X L step (x, g) e (y, g') -> sub X L y f g'.
+Proof.
+  intros f g g' X L step x y e Hsub Hred.
+  assert (exists h : F, h = all e f) as Heq by eauto.
+  destruct Heq as [ h Heq ] ; rewrite <- Heq in *.
+  revert Heq Hred ; revert e f g' ; induction Hsub ;
+    intros e f' g' Heq Hred ; rewrite Heq in *.
+  inversion Hred ; apply sub_refl || auto.
+  assert (e = e) by auto ; contradiction.
+  inversion Hred.
+  apply IHHsub with (f := f') in H4 ; auto.
+  apply IHHsub with (f := f') in H4 ; auto.
+  apply sub_conj_left ; auto.
+  inversion Hred.
+  apply IHHsub with (f := f') in H6 ; auto.
+  apply sub_trans with g'0 ; auto.
+  apply IHHsub with (f := f') in H6 ; auto.
+  apply sub_conj_right ; auto.
+  inversion Hred ; contradiction || auto.
+  apply IHHsub with (f := f') in H7 ; auto.
+  inversion Hred.
+  apply IHHsub with (f := f') in H3 ; auto.
+  apply sub_box.
+  apply sub_trans with f'0 ; auto.
+  apply IHHsub with (f := f') in H3 ; auto.
+  apply sub_conj_right ; auto.
+Qed.
+
+(* []f as a sub-formula is constant under (x, g) -(e)->0 (y', g') *)
+Lemma sub_box_red : forall (X : Set) (L : X -> P -> Prop) 
+  (step : X -> E -> X -> Prop) (x y : X) (e : E) (f g g' : F),
+  sub X L x (box f) g -> zero X L step (x, g) e (y, g') -> sub X L y (box f) g'.
+Proof.
+  intros X L step x y e f g g' Hsub Hred ; assert (exists h : F, h = box f) as Heq by eauto.
+  destruct Heq as [ h Heq ] ; rewrite <- Heq in *.
+  revert Heq Hred ; revert f g' ; induction Hsub ;
+    intros f' g' Heq Hred ; rewrite Heq in *.
+  inversion Hred ; [ apply sub_refl | ].
+  apply sub_conj_left ; apply sub_refl.
+  inversion Hred.
+  apply IHHsub with (f := f') in H4 ; auto.
+  apply IHHsub with (f := f') in H4 ; auto.
+  apply sub_conj_left ; auto.
+  inversion Hred.
+  apply IHHsub with (f := f') in H6 ; auto.
+  apply sub_trans with g'0 ; auto.
+  apply IHHsub with (f := f') in H6 ; auto.
+  apply sub_conj_right ; auto.
+  inversion Hred ; contradiction || auto.
+  apply IHHsub with (f := f') ; auto.
+  inversion Hred.
+  apply IHHsub with (f := f') in H3 ; auto.
+  apply sub_box ; apply sub_trans with f'0 ; auto.
+  apply sub_conj_right ; auto.
+  apply IHHsub with (f := f') ; auto.
+Qed.
+
+(* If []f is a sub-formula of g and (x, g) -->*n (x', g') then f \in sub (x',g') *)
+Lemma sub_trans_box : forall (X : Set) (L : X -> P -> Prop) (step : X -> E -> X -> Prop) 
+  (x x' : X) (f g g' : F) (n : nat), sub X L x (box f) g ->
+  trans (X * F) (rel n X L step) (x, g) (x', g') -> sub X L x' f g'.
+Proof.
+  intros X L step x x' f g g' n Hsub Htrans.
+  assert (exists xg : X * F, xg = (x, g)) as Heq by eauto.
+  assert (exists xg' : X * F, xg' = (x', g')) as Heq' by eauto.
+  destruct Heq as [ xg Heq ] ; rewrite <- Heq in *.
+  destruct Heq' as [ xg' Heq' ] ; rewrite <- Heq' in *.
+  assert (sub X L x' (box f) g') as Hsub'.
+  revert Heq Heq' Hsub ; revert x g x' g'.
+  induction Htrans ; intros z g z' g' Heq Heq' Hsub.
+  rewrite Heq in Heq' ; inversion Heq'.
+  replace z with z' in * by auto ; replace g with g' in * by auto ; auto.
+  rewrite Heq in * ; destruct y as [ y h ].
+  apply rel_impl_zero in H ; apply sub_box_red with (y := y) (f := f) in H ; auto.
+  apply IHHtrans with (x'0 := z') (g' := g') in H ; auto.
+  apply sub_box_in in Hsub' ; auto.
+Qed.
+
+(* Validity of B-formulas only depends on labeling *)
+Lemma bval_iff : forall (b : B) (X : Set) (L : X -> P -> Prop) (x : X) (g : F),
+  bval X L x b <-> bval (X * F) (fun xf => L (fst xf)) (x, g) b.
+Proof.
+  intro b ; induction b ; intros X L x g ; split ; intro H ;
+    solve [ simpl in * ; tauto ] || idtac.
+  simpl in H ; destruct H ; split ; [ apply IHb1 | apply IHb2 ] ; auto.
+  simpl in H ; destruct H as [ Hb1 Hb2 ].
+  apply IHb1 in Hb1 ; apply IHb2 in Hb2 ; split ; auto.
+  simpl in H ; destruct H ; [ left | right ] ; auto.
+  apply IHb1 ; auto.
+  apply IHb2 ; auto.
+  simpl in H ; destruct H as [ Hb1 | Hb2 ].
+  apply IHb1 in Hb1 ; left ; auto.
+  apply IHb2 in Hb2 ; right ; auto.
+  simpl ; intro H' ; simpl in H ; apply H ; apply IHb in H' ; auto.
+  simpl in * ; intro H' ; apply H ; apply IHb ; auto.
+Qed.
+
+(* 
+ * Prove that if synthesizability holds at every
+ * reachable state then the synthesis result satisfies
+ * the synthesized control objective
+ *)
+Theorem validity : forall (n : nat) (X : Set) (L : X -> P -> Prop)
+  (step : X -> E -> X -> Prop) (x : X) (f : F),
+  complete n X L step (x, f) -> fval (S (klts X L step x) f n) f.
+Proof.
+  intros n X L step x f ; assert (sub X L x f f) as H by ( apply sub_refl ).
+  revert H ; revert x ; generalize f at 2 3 4 as g.
+  induction f ; intros g x Hsub Hcomplete ;
+    assert (syn X L (rel n X L step) (x, g) g) as Hsyn by
+    ( apply Hcomplete ; apply trans_refl ).
+  apply sub_syn with (f := basic b) in Hsyn ; auto.
+  inversion Hsyn ; simpl ; apply bval_iff ; auto.
+  apply sub_conj in Hsub ; destruct Hsub as [ Hf1 Hf2 ].
+  split ; [ apply IHf1 | apply IHf2 ] ; auto.
   destruct (classic (bval X L x b)) as [ Hbval | Hnot_bval ].
-  exists (basic true) ; apply red_or_left ; auto.
-  destruct IHf as [ f' Hred ].
-  exists f' ; apply red_or_right ; auto.
-  destruct (classic (e = e0)) as [ H | H ].
-  rewrite <- H in * ; exists f ; apply red_all_pos ; auto.
-  exists (basic true) ; apply red_all_neg ; auto.
-  exists (basic true) ; apply red_ex_neg ; auto.
-  destruct IHf as [ f' Hred ].
-  exists (conj (box f) f') ; apply red_box ; auto.
-  exists (basic true) ; apply red_diam.
-  exists (basic true) ; apply red_can.
-  exists (basic true) ; apply red_dlf.
+  simpl ; left ; apply bval_iff ; auto.
+  apply sub_disj_not in Hsub ; auto.
+  right ; apply IHf ; auto.
+  simpl ; intros xg' Hstep ; destruct xg' as [ x' g' ].
+  assert (zero X L step (x, g) e (x', g')) as Hred.
+  apply rel_impl_zero in Hstep ; auto.
+  apply sub_all with (f := f) (y := x') in Hred ; auto.
+  apply IHf ; auto.
+  intros xf' Htrans ; apply Hcomplete.
+  apply trans_closed with (x', g') e ; auto.
+  assert (syn X L (rel n X L step) (x, g) (ex e f)) as Hex.
+  apply sub_syn with g ; auto.
+  inversion Hex ; exists (x', g') ; split ; auto.
+  apply IHf ; auto.
+  intros xg' Htrans ; apply Hcomplete.
+  apply trans_closed with (x', g') e ; auto.
+  simpl ; intros xg' Htrans ; destruct xg' as [ x' g' ].
+  apply IHf ; auto.
+  apply sub_trans_box with (f := f) in Htrans ; auto.
+  intros xg' Htrans' ; apply Hcomplete.
+  apply trans_cat with (x', g') ; auto.
+  assert (syn X L (rel n X L step) (x, g) (diam b)) as H.
+  apply sub_syn with (g := g) ; auto.
+  inversion H ; exists (x', g') ; split ; auto.
+  apply bval_iff ; auto.
+  assert (syn X L (rel n X L step) (x, g) (can e)) as H.
+  apply sub_syn with (g := g) ; auto.
+  inversion H ; exists (x', g') ; auto.
+  assert (syn X L (rel n X L step) (x, g) dlf) as H.
+  apply sub_syn with (g := g) ; auto.
+  inversion H ; exists e ; exists (x', g') ; auto.
 Qed.
 
+(* If x -(e)-> x' then an f' such that (x, f) -(e)-> (x', f') exists *)
+Lemma zero_ex : forall (f : F) (X : Set) (L : X -> P -> Prop)
+  (step : X -> E -> X -> Prop) (x y : X) (e : E), step x e y ->
+  exists f' : F, zero X L step (x, f) e (y, f').
+Proof.
+  intro f ; induction f ; intros X L step x y e' Hstep.
+  exists (basic true) ; apply zero_basic ; auto.
+  destruct (IHf1 X L step x y e') as [ f1' Hred_f1 ] ; auto.
+  destruct (IHf2 X L step x y e') as [ f2' Hred_f2 ] ; auto.
+  destruct (classic (sub X L y f2' f1')) as [ Hsub | Hnot_sub ].
+  exists f1' ; apply zero_conj_incl with f2' ; auto.
+  exists (conj f1' f2') ; apply zero_conj_excl ; auto.
+  destruct (classic (bval X L x b)) as [ Hbval | Hnot_bval ].
+  exists (basic true) ; apply zero_disj_left ; auto.
+  destruct (IHf X L step x y e') as [ f' Hred ] ; auto.
+  exists f' ; apply zero_disj_right ; auto.
+  destruct (classic (e = e')) as [ Heq | Hnot_eq ].
+  rewrite Heq ; exists f ; apply zero_all_pos ; auto.
+  exists (basic true) ; apply zero_all_neg ; auto.
+  exists (basic true) ; apply zero_ex_neg ; auto.
+  destruct (IHf X L step x y e') as [ f' Hred ] ; auto.
+  destruct (classic (sub X L y f' f)) as [ Hsub | Hnot_sub ].
+  exists (box f) ; apply zero_box_incl with f' ; auto.
+  exists (conj (box f) f') ; apply zero_box_excl ; auto.
+  exists (basic true) ; apply zero_diam ; auto.
+  exists (basic true) ; apply zero_can ; auto.
+  exists (basic true) ; apply zero_dlf ; auto.
+Qed.
+
+(* If (x, f) -(e)->0 (x', f') then (x, f) -(e)->n (x', f') if e is uncontrollable *)
 Lemma unctrl_ex : forall (n : nat) (X : Set) (L : X -> P -> Prop)
-  (step : X -> E -> X -> Prop) (x x' : X) (f f' : F) (e : E),
-  step x e x' -> red X L x f e f' -> U e -> rel n X L step (x, f) e (x', f').
+  (step : X -> E -> X -> Prop) (x x' : X) (e : E) (f f' : F), U e ->
+  zero X L step (x, f) e (x', f') -> rel n X L step (x, f) e (x', f').
 Proof.
-  intro n ; induction n ; 
-    intros X L step x x' f f' e Hstep Hred HU.
-  simpl ; split ; auto.
+  intro n ; induction n ; intros X L step x x' e f f' HU Hzero.
+  simpl ; unfold rel ; simpl ; auto.
   simpl ; split ; auto.
 Qed.
 
-Theorem controllability : forall (X : Set) (L : X -> P -> Prop)
-  (step : X -> E -> X -> Prop) (x : X) (f : F) (n : nat),
-  pbis (S (klts X L step x) f n) (klts X L step x).
+(* 
+ * Prove that the synthesis result is related to the original 
+ * model via partial bisimulation, which implies controllability
+ *)
+Theorem controllability : forall (k : K) (f : F) (n : nat),
+  pbis (S k f n) k.
 Proof.
-  intros X L step x f n.
+  intros k f n ; destruct k as [ X L step x ].
   exists (fun yg y => fst yg = y) ; split ; auto.
-  intros yg y' H ; destruct yg as [ y g ] ; simpl in H.
-  rewrite <- H in * ; split ; [ simpl ; tauto | split ] ; clear H y'.
-  intros e yg' Hrel ; destruct yg' as [ y' g' ].
-  apply rel_impl_step_red in Hrel ; destruct Hrel as [ Hstep _ ].
-  exists y' ; repeat split ; simpl ; auto.
-  intros e y' HU Hstep ; destruct (red_ex X L y g e) as [ g' Hred ].
-  exists (y', g') ; repeat split ; auto.
-  apply unctrl_ex ; auto.
+  intros y' y Heq ; destruct y' as [ y' g ].
+  simpl in Heq ; rewrite Heq in * ; clear Heq y'.
+  split ; [ simpl ; tauto | split ].
+  intros e zg' Hrel ; destruct zg' as [ z g' ].
+  apply rel_impl_zero in Hrel ; apply zero_impl_step in Hrel.
+  exists z ; split ; simpl ; auto.
+  intros e z HU Hstep ; destruct (zero_ex g X L step y z e) as [ g' Hred ] ; auto.
+  exists (z, g') ; split ; apply unctrl_ex || auto ; auto.
 Qed.
 
+(* 
+ * If k = (X,L,-->,x) and k |= f and x -(e)-> x' then there
+ * exists f' such that (x, f) -(e)->0 (x', f') and (X,L,-->,x') |= f'
+ *) 
+Lemma val_next : forall (f : F) (X : Set) (L : X -> P -> Prop)
+  (step : X -> E ->  X -> Prop) (x x' : X) (e : E), step x e x' ->
+  fval (klts X L step x) f -> exists f' : F, zero X L step (x, f) e (x', f') /\ 
+  fval (klts X L step x') f'.
+Proof.
+  intro f ; induction f ; intros X L step x x' e' Hstep Hval.
+  exists (basic true) ; split ; apply zero_basic || simpl ; auto.
+  simpl in Hval ; destruct Hval as [ Hf1 Hf2 ].
+  apply IHf1 with (x' := x') (e := e') in Hf1 ; auto.
+  apply IHf2 with (x' := x') (e := e') in Hf2 ; auto.
+  destruct Hf1 as [ f1' [ Hred_f1 Hval_f1 ] ].
+  destruct Hf2 as [ f2' [ Hred_f2 Hval_f2 ] ].
+  destruct (classic (sub X L x' f2' f1')) as [ Hsub | Hnot_sub ].
+  exists f1' ; split ; [ apply zero_conj_incl with f2' ; auto | auto ].
+  exists (conj f1' f2') ; split.
+  apply zero_conj_excl ; auto.
+  split ; auto.
+  simpl in Hval ; destruct Hval as [ Hbval | Hval ].
+  exists (basic true) ; split ; simpl ; auto.
+  apply zero_disj_left ; auto.
+  destruct (classic (bval X L x b)) as [ Hbval | Hnot_bval ].
+  exists (basic true) ; split ; simpl ; auto.
+  apply zero_disj_left ; auto.
+  apply IHf with (x' := x') (e := e') in Hval ; auto.
+  destruct Hval as [ f' [ Hred Hval ] ].
+  exists f' ; split ; auto.
+  apply zero_disj_right ; auto.
+  destruct (classic (e = e')) as [ Heq | Hnot_eq ].
+  rewrite <- Heq in * ; exists f ; split ; auto.
+  apply zero_all_pos ; auto.
+  exists (basic true) ; split ; simpl ; auto.
+  apply zero_all_neg ; auto.
+  exists (basic true) ; split ; simpl ; auto.
+  apply zero_ex_neg ; auto.
+  assert (fval (klts X L step x) f) as Hval_f.
+  apply Hval ; apply trans_refl.
+  apply IHf with (x' := x') (e := e') in Hval_f ; auto.
+  destruct Hval_f as [ f' [ Hred Hval_f' ] ].
+  destruct (classic (sub X L x' f' f)) as [ Hsub | Hnot_sub ].
+  exists (box f) ; split ; auto.
+  apply zero_box_incl with f' ; auto.
+  intros x'' Htrans ; apply Hval.
+  apply trans_closed with x' e' ; auto.
+  exists (conj (box f) f') ; split ; auto.
+  apply zero_box_excl ; auto.
+  split ; auto.
+  intros x'' Htrans ; apply Hval.
+  apply trans_closed with x' e' ; auto.
+  exists (basic true) ; split ; simpl ; auto.
+  apply zero_diam ; auto.
+  exists (basic true) ; split ; simpl ; auto.
+  apply zero_can ; auto.
+  exists (basic true) ; split ; simpl ; auto.
+  apply zero_dlf ; auto.
+Qed.
 
-Lemma pbis_bval : forall (b : B) (X' X : Set) (L' : X' -> P -> Prop)
+(* Synthesizability in synthesis step n+1 implies the same in step n *)
+Lemma syn_less : forall (f g : F) (n : nat) (X : Set) (L : X -> P -> Prop)
+  (step : X -> E -> X -> Prop) (x : X), syn X L (rel (Datatypes.S n) X L step) (x, g) f ->
+  syn X L (rel n X L step) (x, g) f.
+Proof.
+  assert (forall (n : nat) (X : Set) (L : X -> P -> Prop)
+    (step : X -> E -> X -> Prop) (x x' : X) (g g' : F),
+    trans (X * F) (rel (Datatypes.S n) X L step) (x, g) (x', g') ->
+    trans (X * F) (rel n X L step) (x, g) (x', g')) as Htrans.
+  intros n X L step x x' g g' Htrans.
+  assert (exists xg : X * F, xg = (x, g)) as Heq by eauto.
+  assert (exists xg' : X * F, xg' = (x', g')) as Heq' by eauto.
+  destruct Heq as [ xg Heq ] ; rewrite <- Heq in *.
+  destruct Heq' as [ xg' Heq' ] ; rewrite <- Heq' in *.
+  revert Heq Heq' ; revert x g x' g'.
+  induction Htrans ; intros z g z' g' Heq Heq' ; apply trans_refl || auto.
+  rewrite Heq in * ; destruct y as [ y h ] ; rewrite Heq' in *.
+  apply trans_closed with (y, h) e ; auto.
+  apply IHHtrans with y h z' g' ; simpl in H ; tauto.
+  simpl in H ; tauto.
+  intro f ; induction f ; intros g n X L step x Hsyn.
+  inversion Hsyn ; apply syn_basic ; auto.
+  inversion Hsyn ; apply syn_conj ; auto.
+  inversion Hsyn ; [ apply syn_disj_left ; auto | ].
+  apply syn_disj_right ; auto.
+  apply syn_all.
+  inversion Hsyn ; apply syn_ex with x' g' ; auto.
+  simpl in * ; tauto.
+  inversion Hsyn ; apply syn_box ; auto.
+  inversion Hsyn ; apply syn_diam with x' g' ; auto.
+  inversion Hsyn ; apply syn_can with x' g'.
+  simpl in * ; tauto.
+  inversion Hsyn ; apply syn_dlf with x' e g'.
+  simpl in * ; tauto.
+Qed.
+
+(* 
+ * If (x, f) -(e)->0 (x', f') and for all (x', f') -->*n (x'', f'')
+ * synthesizability holds, then we can derive (x, f) -(e)->n (x', f')
+ *)
+Lemma rel_ex : forall (n : nat) (X : Set) (L : X -> P -> Prop) 
+  (step : X -> E -> X -> Prop) (x x' : X) (e : E) (f f' : F),
+  (forall (x'' : X) (f'' : F), trans (X * F) (unctrl (X * F) (rel n X L step)) (x', f') (x'', f'') ->
+    syn X L (rel n X L step) (x'', f'') f'') ->
+  zero X L step (x, f) e (x', f') -> rel n X L step (x, f) e (x', f').
+Proof.
+  assert (forall (X : Set) (L : X -> P -> Prop) (step : X -> E -> X -> Prop)
+    (x x' : X) (g g' : F) (n : nat), 
+    trans (X * F) (unctrl (X * F) (rel n X L step)) (x, g) (x', g') ->
+    trans (X * F) (unctrl (X * F) (rel (Datatypes.S n) X L step)) (x, g) (x', g')) as Htrans.
+  intros X L step x x' g g' n Htrans.
+  assert (exists xg : X * F, xg = (x, g)) as Heq by eauto.
+  assert (exists xg' : X * F, xg' = (x', g')) as Heq' by eauto.
+  destruct Heq as [ xg Heq ] ; rewrite <- Heq in *.
+  destruct Heq' as [ xg' Heq' ] ; rewrite <- Heq' in *.
+  revert Heq Heq' ; revert x g x' g'.
+  induction Htrans ; intros z g z' g' Heq Heq' ; apply trans_refl || auto.
+  rewrite Heq in * ; destruct y as [ y h ] ; rewrite Heq' in *.
+  apply trans_closed with (y, h) e ; auto.
+  apply IHHtrans with y h z' g' ; simpl in H ; tauto.
+  unfold unctrl in * ; simpl ; tauto.
+  intro n ; induction n ; intros X L step x x' e f f' H Hred.
+  simpl ; unfold rel ; simpl ; auto.
+  simpl ; split ; [ apply IHn ; auto | ].
+  intros x'' f'' Htrans' ; apply syn_less ; apply H.
+  apply Htrans ; auto.
+  right ; intros xf'' Htrans' ; destruct xf'' as [ x'' f'' ].
+  simpl ; apply syn_less ; apply H.
+  apply Htrans ; auto.
+Qed.
+
+(* 
+ * If (X,L,-->,x) |= f and (x, f) -(e)-> (x',f') and 
+ * event e is uncontrollable, then (X,L,-->,x') |= f'
+ *)
+Lemma wf_next : forall (f f' : F) (X : Set) (L : X -> P -> Prop)
+  (step : X -> E ->  X -> Prop) (x x' : X) (e : E), step x e x' ->
+  fval (klts X L step x) f -> wf f -> U e -> 
+  zero X L step (x, f) e (x', f') -> fval (klts X L step x') f'.
+Proof.
+  intro f ; induction f ; 
+    intros f' X L step x x' e' Hstep Hval Hwf HU Hred ;
+    solve [ inversion Hred ; simpl in * ; tauto ] || idtac.
+  inversion Hred ; simpl in Hval ; destruct Hval.
+  destruct (classic (sub X L x' g' f')) as [ Hsub | Hnot_sub ].
+  apply IHf1 with x e' ; simpl in * ; tauto.
+  apply IHf1 in H4 ; simpl in * ; tauto || auto.
+  apply IHf1 in H4 ; simpl in * ; tauto || auto.
+  apply IHf2 in H6 ; simpl in * ; tauto || auto.
+  inversion Hred ; simpl ; auto.
+  simpl in Hval ; destruct Hval as [ Hbval | Hval ] ;
+    contradiction || auto.
+  apply IHf with x e' ; simpl in * ; tauto.
+  inversion Hred ; [ replace e with e' in * by auto | simpl ; auto ].
+  replace f with f' in * by auto ; simpl in * ; auto.
+  inversion Hred ; [ replace e with e' in * by auto | simpl ; auto ].
+  replace f with f' in * by auto ; simpl in * ; auto.
+  destruct Hwf ; contradiction.
+  inversion Hred.
+  intros x'' Htrans ; apply Hval.
+  apply trans_closed with x' e' ; auto.
+  split ; auto.
+  intros x'' Htrans ; apply Hval.
+  apply trans_closed with x' e' ; auto.
+  apply IHf with x e' ; simpl in * ; auto.
+  apply Hval ; apply trans_refl.
+Qed.
+
+(* The well-formedness test is stable under (x, f) -(e)->0 (x',f') *)
+Lemma wf_zero : forall (f : F) (X : Set) (L : X -> P -> Prop) 
+  (step : X -> E -> X -> Prop) (x y : X) (f' : F) (e : E),
+  wf f -> zero X L step (x, f) e (y, f') -> wf f'.
+Proof.
+  intro f ; induction f ; intros X L step x y f' e' Hwf Hred ;
+    solve [ inversion Hred ; simpl ; auto ] || auto.
+  simpl in Hwf ; destruct Hwf ; inversion Hred.
+  apply IHf1 in H6 ; auto.
+  apply IHf1 in H6 ; apply IHf2 in H8 ; simpl ; tauto.
+  simpl in Hwf ; inversion Hred ; simpl ; auto.
+  apply IHf in H6 ; auto.
+  inversion Hred ; simpl in Hwf ; simpl ; auto.
+  replace f' with f in * ; auto.
+  inversion Hred ; simpl in Hwf ; simpl ; auto.
+  replace f' with f in * ; tauto.
+  inversion Hred ; auto.
+  apply IHf in H3 ; simpl ; auto.
+Qed.
+
+(* Partial bisimulation implies validity for B-formulas *)
+Lemma pbis_bval : forall (b : B) (X X' : Set) (L' : X' -> P -> Prop)
   (L : X -> P -> Prop) (step' : X' -> E -> X' -> Prop)
   (step : X -> E -> X -> Prop) (x' : X') (x : X),
   pbis (klts X' L' step' x') (klts X L step x) ->
   (bval X' L' x' b <-> bval X L x b).
 Proof.
-  intro b ; induction b ; intros X' X L' L step' step x' x Hpbis ; 
-    split ; intro H ; solve [ simpl in * ; tauto ] || idtac.
-  destruct Hpbis as [ R [ HinR HrelR ] ].
-  apply HrelR in HinR ; apply HinR in H ; simpl ; auto.
-  destruct Hpbis as [ R [ HinR HrelR ] ].
-  apply HrelR in HinR ; apply HinR in H ; simpl ; auto.
-  apply IHb in Hpbis ; intro H' ; apply H ; tauto.
-  apply IHb in Hpbis ; intro H' ; apply H ; tauto.
-  simpl in H ; destruct H as [ Hb1 Hb2 ] ; split ; auto.
-  apply IHb1 in Hpbis ; apply Hpbis ; auto.
-  apply IHb2 in Hpbis ; apply Hpbis ; auto.
-  simpl in H ; destruct H as [ Hb1 Hb2 ] ; split ; auto.
-  apply IHb1 in Hpbis ; apply Hpbis ; auto.
-  apply IHb2 in Hpbis ; apply Hpbis ; auto.
-  simpl in H ; destruct H as [ Hb1 | Hb2 ] ; auto.
-  left ; apply IHb1 in Hpbis ; apply Hpbis ; auto.
-  right ; apply IHb2 in Hpbis ; apply Hpbis ; auto.
-  simpl in H ; destruct H as [ Hb1 | Hb2 ] ; auto.
-  left ; apply IHb1 in Hpbis ; apply Hpbis ; auto.
-  right ; apply IHb2 in Hpbis ; apply Hpbis ; auto.
+  intro b ; induction b ; 
+    intros X X' L' L step' step x' x Hpbis ; split ; intro H ;
+    solve [ simpl in * ; tauto ] || idtac.
+  simpl in * ; destruct Hpbis as [ R [ HinR HrelR ] ].
+  apply HrelR in HinR ; apply HinR in H ; auto.
+  simpl in * ; destruct Hpbis as [ R [ HinR HrelR ] ].
+  apply HrelR in HinR ; apply HinR in H ; auto.
+  simpl in H ; destruct H as [ Hb1 Hb2 ] ; 
+    simpl ; split ; auto.
+  apply IHb1 in Hpbis ; tauto.
+  apply IHb2 in Hpbis ; tauto.
+  simpl in H ; destruct H as [ Hb1 Hb2 ] ; 
+    simpl ; split ; auto.
+  apply IHb1 in Hpbis ; tauto.
+  apply IHb2 in Hpbis ; tauto.
+  simpl in H ; destruct H as [ Hb1 | Hb2 ] ; simpl ; auto.
+  left ; apply IHb1 in Hpbis ; tauto.
+  right ; apply IHb2 in Hpbis ; tauto.
+  simpl in H ; destruct H as [ Hb1 | Hb2 ] ; simpl ; auto.
+  left ; apply IHb1 in Hpbis ; tauto.
+  right ; apply IHb2 in Hpbis ; tauto.
+  simpl ; intro H' ; simpl in H ; apply H.
+  apply IHb in Hpbis ; tauto.
+  simpl ; intro H' ; simpl in H ; apply H.
+  apply IHb in Hpbis ; tauto.
 Qed.
 
-Lemma pbis_sub : forall (f g : F) (X' X : Set) (L' : X' -> P -> Prop)
+(* 
+ * Since partial bisimulation implies the validity of
+ * B-formulas, and since the sub-formula predicate depends
+ * upon B-formula validity (for the b \/ g case), partial
+ * bisimulation also implies sub-formulas 
+ *)
+Lemma pbis_sub : forall (X X' : Set) (L' : X' -> P -> Prop)
   (L : X -> P -> Prop) (step' : X' -> E -> X' -> Prop)
-  (step : X -> E -> X -> Prop) (x' : X') (x : X),
+  (step : X -> E -> X -> Prop) (x' : X') (x : X) (f g : F),
   pbis (klts X' L' step' x') (klts X L step x) ->
   (sub X' L' x' f g <-> sub X L x f g).
 Proof.
-  intros f g X' X L' L step' step x' x Hpbis ; split ;
-    intro H ; induction H ; solve [ tauto ] || apply sub_refl || 
-    solve [ apply sub_and_left ; auto ] || solve [ apply sub_and_right ; auto ] || 
-    solve [ apply sub_box ; auto ] || apply sub_or ; auto.
+  intros X X' L' L step' step x' x f g Hpbis ;
+    split ; intro Hsub ; induction Hsub ; auto.
+  apply sub_refl.
+  apply sub_conj_left ; auto.
+  apply sub_conj_right ; auto.
+  apply sub_disj ; auto.
   intro H' ; apply H ; apply pbis_bval with (b := b) in Hpbis ; tauto.
+  apply sub_box ; auto.
+  apply sub_refl.
+  apply sub_conj_left ; auto.
+  apply sub_conj_right ; auto.
+  apply sub_disj ; auto.
   intro H' ; apply H ; apply pbis_bval with (b := b) in Hpbis ; tauto.
+  apply sub_box ; auto.
 Qed.
 
-Lemma pbis_red : forall (f f' : F) (e : E) (X' X : Set) (L' : X' -> P -> Prop)
+(* Partial bisimulation implies (x, f) -(e)->0 (x', f') *)
+Lemma pbis_zero : forall (f : F) (X X' : Set) (L' : X' -> P -> Prop)
   (L : X -> P -> Prop) (step' : X' -> E -> X' -> Prop)
-  (step : X -> E -> X -> Prop) (x' : X') (x : X),
-  pbis (klts X' L' step' x') (klts X L step x) ->
-  (red X' L' x' f e f' <-> red X L x f e f').
+  (step : X -> E -> X -> Prop) (x' y' : X') (x y : X) (f' : F) (e : E),
+  pbis (klts X' L' step' x') (klts X L step x) -> step' x' e y' ->
+  pbis (klts X' L' step' y') (klts X L step y) -> step x e y ->
+  (zero X' L' step' (x', f) e (y', f') <-> zero X L step (x, f) e (y, f')).
 Proof.
-  intros f f' e X' X L' L step' step x' x Hpbis ;
-    split ; intro H ; induction H ; solve [ apply red_basic ] ||
-    solve [ apply red_and ; auto ] || solve [ apply red_all_pos ] ||
-    solve [ apply red_all_neg ; auto ] || solve [ apply red_ex_pos ] ||
-    solve [ apply red_ex_neg ] || solve [ apply red_box ; auto ] || 
-    solve [ apply red_diam ] || solve [ apply red_can ] ||
-    solve [ apply red_dlf ] || idtac.
-  apply red_or_left ; auto.
+  intro f ; induction f ; intros X X' L' L step' step x' y' x y f' e' Hpbis Hstep' Hpbis' Hstep.
+  split ; intro H ; inversion H ; apply zero_basic ; auto.
+  split ; intro H ; inversion H.
+  apply zero_conj_incl with g' ; auto.
+  apply IHf1 with (X := X) (X' := X') (L := L) (L' := L')
+    (step := step) (step' := step') (x' := x') (x := x)
+    (y' := y') (y := y) (e := e') (f' := f') in Hpbis ; tauto.
+  apply IHf2 with (X := X) (X' := X') (L := L) (L' := L')
+    (step := step) (step' := step') (x' := x') (x := x)
+    (y' := y') (y := y) (e := e') (f' := g') in Hpbis ; tauto.
+  apply pbis_sub with (f := g') (g := f') in Hpbis' ; tauto.
+  apply zero_conj_excl ; auto.
+  apply IHf1 with (X := X) (X' := X') (L := L) (L' := L')
+    (step := step) (step' := step') (x' := x') (x := x)
+    (y' := y') (y := y) (e := e') (f' := f'0) in Hpbis ; tauto.
+  apply IHf2 with (X := X) (X' := X') (L := L) (L' := L')
+    (step := step) (step' := step') (x' := x') (x := x)
+    (y' := y') (y := y) (e := e') (f' := g') in Hpbis ; tauto.
+  intro H' ; apply H8.
+  apply pbis_sub with (f := g') (g := f'0) in Hpbis' ; tauto.
+  apply zero_conj_incl with g' ; auto.
+  apply IHf1 with (X := X) (X' := X') (L := L) (L' := L')
+    (step := step) (step' := step') (x' := x') (x := x)
+    (y' := y') (y := y) (e := e') (f' := f') in Hpbis ; tauto.
+  apply IHf2 with (X := X) (X' := X') (L := L) (L' := L')
+    (step := step) (step' := step') (x' := x') (x := x)
+    (y' := y') (y := y) (e := e') (f' := g') in Hpbis ; tauto.
+  apply pbis_sub with (f := g') (g := f') in Hpbis' ; tauto.
+  apply zero_conj_excl ; auto.
+  apply IHf1 with (X := X) (X' := X') (L := L) (L' := L')
+    (step := step) (step' := step') (x' := x') (x := x)
+    (y' := y') (y := y) (e := e') (f' := f'0) in Hpbis ; tauto.
+  apply IHf2 with (X := X) (X' := X') (L := L) (L' := L')
+    (step := step) (step' := step') (x' := x') (x := x)
+    (y' := y') (y := y) (e := e') (f' := g') in Hpbis ; tauto.
+  intro H' ; apply H8.
+  apply pbis_sub with (f := g') (g := f'0) in Hpbis' ; tauto.
+  split ; intro H ; inversion H.
+  apply zero_disj_left ; auto.
   apply pbis_bval with (b := b) in Hpbis ; tauto.
-  apply red_or_right ; auto.
-  apply pbis_bval with (b := b) in Hpbis ; tauto.  
-  apply red_or_left ; auto.
+  apply zero_disj_right ; auto.
+  intro H' ; apply H4.
   apply pbis_bval with (b := b) in Hpbis ; tauto.
-  apply red_or_right ; auto.
+  apply IHf with (X := X) (X' := X') (L := L) (L' := L')
+    (step := step) (step' := step') (x' := x') (x := x)
+    (y' := y') (y := y) (e := e') (f' := f') in Hpbis ; try tauto.
+  apply zero_disj_left ; auto.
   apply pbis_bval with (b := b) in Hpbis ; tauto.
+  apply zero_disj_right ; auto.
+  intro H' ; apply H4.
+  apply pbis_bval with (b := b) in Hpbis ; tauto.
+  apply IHf with (X := X) (X' := X') (L := L) (L' := L')
+    (step := step) (step' := step') (x' := x') (x := x)
+    (y' := y') (y := y) (e := e') (f' := f') in Hpbis ; try tauto.
+  split ; intro H ; inversion H.
+  apply zero_all_pos ; auto.
+  apply zero_all_neg ; auto.
+  apply zero_all_pos ; auto.
+  apply zero_all_neg ; auto.
+  split ; intro H ; inversion H.
+  apply zero_ex_pos ; auto.
+  apply zero_ex_neg ; auto.
+  apply zero_ex_pos ; auto.
+  apply zero_ex_neg ; auto.
+  split ; intro H ; inversion H.
+  apply zero_box_incl with f'0 ; auto.
+  apply IHf with (X := X) (X' := X') (L := L) (L' := L')
+    (step := step) (step' := step') (x' := x') (x := x)
+    (y' := y') (y := y) (e := e') (f' := f'0) in Hpbis ; try tauto.
+  apply pbis_sub with (f := f'0) (g := f) in Hpbis' ; tauto.
+  apply zero_box_excl ; auto.
+  apply IHf with (X := X) (X' := X') (L := L) (L' := L')
+    (step := step) (step' := step') (x' := x') (x := x)
+    (y' := y') (y := y) (e := e') (f' := f'0) in Hpbis ; try tauto.
+  intro H' ; apply H6.
+  apply pbis_sub with (f := f'0) (g := f) in Hpbis' ; tauto.
+  apply zero_box_incl with f'0 ; auto.
+  apply IHf with (X := X) (X' := X') (L := L) (L' := L')
+    (step := step) (step' := step') (x' := x') (x := x)
+    (y' := y') (y := y) (e := e') (f' := f'0) in Hpbis ; try tauto.
+  apply pbis_sub with (f := f'0) (g := f) in Hpbis' ; tauto.
+  apply zero_box_excl ; auto.
+  apply IHf with (X := X) (X' := X') (L := L) (L' := L')
+    (step := step) (step' := step') (x' := x') (x := x)
+    (y' := y') (y := y) (e := e') (f' := f'0) in Hpbis ; try tauto.
+  intro H' ; apply H6.
+  apply pbis_sub with (f := f'0) (g := f) in Hpbis' ; tauto.
+  split ; intro H ; inversion H ; apply zero_diam ; auto.
+  split ; intro H ; inversion H ; apply zero_can ; auto.
+  split ; intro H ; inversion H ; apply zero_dlf ; auto.
 Qed.
 
-Lemma val_next : forall (f : F) (X : Set) (L : X -> P -> Prop)
-  (step : X -> E -> X -> Prop) (x x' : X) (e : E),
-  val (klts X L step x) f -> step x e x' -> exists f' : F,
-  red X L x f e f' /\ val (klts X L step x') f'.
-Proof.
-  intro f ; induction f ; intros X L step x x' e' Hval Hstep.
-  exists (basic true) ; split ; simpl ; apply red_basic || auto.
-  simpl in Hval ; destruct Hval as [ Hf1 Hf2 ].
-  apply IHf1 with (step := step) (x' := x') (e := e') in Hf1 ; auto.
-  apply IHf2 with (step := step) (x' := x') (e := e') in Hf2 ; auto.
-  destruct Hf1 as [ f1' [ Hred_f1 Hval_f1 ] ].
-  destruct Hf2 as [ f2' [ Hred_f2 Hval_f2 ] ].
-  exists (conj f1' f2') ; split ; simpl ; apply red_and || auto ; auto.
-  simpl in Hval ; destruct Hval as [ Hb | Hf ].
-  exists (basic true) ; split ; simpl ; apply red_or_left || auto ; auto.
-  apply IHf with (step := step) (x' := x') (e := e') in Hf ; auto.
-  destruct (classic (bval X L x b)) as [ Hbval | Hnot_bval ].
-  exists (basic true) ; split ; apply red_or_left || auto ; simpl ; auto.
-  destruct Hf as [ f' [ Hred Hval ] ].
-  exists f' ; split ; apply red_or_right || auto ; auto.
-  destruct (classic (e = e')) as [ Heq | Hnot_eq ]. 
-  rewrite <- Heq in * ; exists f ; split ; apply red_all_pos || auto.
-  exists (basic true) ; split ; simpl ; apply red_all_neg || auto ; auto.
-  exists (basic true) ; split ; simpl ; apply red_ex_neg || auto ; auto.
-  assert (val (klts X L step x) f) as Hval'.
-  apply Hval ; apply trans_refl.
-  apply IHf with (step := step) (x' := x') (e := e') in Hval' ; auto.
-  destruct Hval' as [ f' [ Hred Hval' ] ].
-  exists (conj (box f) f') ; split ; apply red_box || auto ; auto.
-  simpl ; split ; auto.
-  intros x'' Htrans ; apply Hval.
-  apply trans_closed with x' e' ; auto.
-  exists (basic true) ; split ; apply red_diam || auto ; simpl ; auto.
-  exists (basic true) ; split ; apply red_can || auto ; simpl ; auto.
-  exists (basic true) ; split ; apply red_dlf || auto ; simpl ; auto.
-Qed.
-
+(* 
+ * If <e>f is a sub-formula of g and if k = (X,L,-->,x)
+ * such that k |= g then there exists (x, g) -(e)->0 (x',g')
+ * such that (X,L,-->,x') |= g' and f is a sub-formula of g'
+ *)
 Lemma ex_next : forall (f g : F) (X : Set) (L : X -> P -> Prop)
-  (step : X -> E -> X -> Prop) (x : X) (e : E),
-  sub X L x (ex e f) g -> val (klts X L step x) g ->
-  exists x' : X, exists g' : F, step x e x' /\
-  red X L x g e g' /\ val (klts X L step x') g' /\
-  sub X L x' f g'.
+  (step : X -> E -> X -> Prop) (x : X) (e : E), 
+  fval (klts X L step x) g -> sub X L x (ex e f) g ->
+  exists x' : X, exists g' : F, zero X L step (x, g) e (x', g') /\
+  fval (klts X L step x') g' /\ sub X L x' f g'.
 Proof.
-  intros f g X L step x e Hsub Hval.
+  intros f g X L step x e Hval Hsub.
   assert (exists h : F, h = ex e f) as Hex by eauto.
   destruct Hex as [ h Heq ] ; rewrite <- Heq in *.
   induction Hsub ; rewrite Heq in *.
-  simpl in Hval ; destruct Hval as [ x' [ Hstep Hval ] ].
-  exists x' ; exists f ; repeat split ; 
-    apply red_ex_pos || apply sub_refl || auto.
+  simpl in Hval ; destruct Hval as [ x' [ Hstep Hval' ] ].
+  exists x' ; exists f ; repeat split ; apply sub_refl || auto.
+  apply zero_ex_pos ; auto.
   simpl in Hval ; destruct Hval as [ Hg Hh ].
-  apply IHHsub in Hg ; auto.
-  destruct Hg as [ x' [ g' [ Hstep [ Hred [ Hval Hsub' ] ] ] ] ].
-  apply val_next with (f := h) (X := X) (L := L) (x := x) 
-    (e := e) (x' := x') (step := step) in Hh ; auto.
-  destruct Hh as [ h' [ Hred' Hval' ] ].
-  exists x' ; exists (conj g' h') ; repeat split ; auto.
-  apply red_and ; auto.
-  apply sub_and_left ; auto.
+  apply IHHsub in Hg ; clear IHHsub ; auto.
+  destruct Hg as [ x' [ g' [ Hred_g [ Hval_g Hsub_g ] ] ] ].
+  apply val_next with (e := e) (x' := x') in Hh ; auto.
+  destruct Hh as [ h' [ Hred_h Hval_h ] ].
+  exists x' ; destruct (classic (sub X L x' h' g')) as [ Hsub' | Hnot_sub ].
+  exists g' ; repeat split ; auto.
+  apply zero_conj_incl with (g' := h') ; auto.
+  exists (conj g' h') ; repeat split ; auto.
+  apply zero_conj_excl ; auto.
+  apply sub_conj_left ; auto.
+  apply zero_impl_step in Hred_g ; auto.
   simpl in Hval ; destruct Hval as [ Hg Hh ].
-  apply IHHsub in Hh ; auto.
-  destruct Hh as [ x' [ h' [ Hstep [ Hred [ Hval Hsub' ] ] ] ] ].
-  apply val_next with (f := g) (X := X) (L := L) (x := x) 
-    (e := e) (x' := x') (step := step) in Hg ; auto.
-  destruct Hg as [ g' [ Hred' Hval' ] ].
-  exists x' ; exists (conj g' h') ; repeat split ; auto.
-  apply red_and ; auto.
-  apply sub_and_right ; auto.
-  simpl in Hval ; destruct Hval as [ Hbval | Hval ] ;
+  apply IHHsub in Hh ; clear IHHsub ; auto.
+  destruct Hh as [ x' [ h' [ Hred_h [ Hval_h Hsub_h ] ] ] ].
+  apply val_next with (e := e) (x' := x') in Hg ; auto.
+  destruct Hg as [ g' [ Hred_g Hval_g ] ].
+  exists x' ; destruct (classic (sub X L x' h' g')) as [ Hsub' | Hnot_sub ].
+  exists g' ; repeat split ; auto.
+  apply zero_conj_incl with (g' := h') ; auto.
+  apply sub_trans with h' ; auto.
+  exists (conj g' h') ; repeat split ; auto.
+  apply zero_conj_excl ; auto.
+  apply sub_conj_right ; auto.
+  apply zero_impl_step in Hred_h ; auto.
+  simpl in Hval ; destruct Hval as [ Hval | Hval ] ;
     contradiction || auto.
-  apply IHHsub in Hval ; auto.
-  destruct Hval as [ x' [ f' [ Hstep [ Hred [ Hval Hsub' ] ] ] ] ].
-  exists x' ; exists f' ; repeat split ; auto.
-  apply red_or_right ; auto.
-  assert (val (klts X L step x) g) as Hval'.
+  apply IHHsub in Hval ; clear IHHsub ; auto.
+  destruct Hval as [ x' [ g' [ Hred [ Hval Hsub' ] ] ] ].
+  exists x' ; exists g' ; repeat split ; auto.
+  apply zero_disj_right ; auto.
+  assert (fval (klts X L step x) g) as Hval'.
   apply Hval ; apply trans_refl.
-  apply IHHsub in Hval' ; auto.
-  destruct Hval' as [ x' [ g' [ Hstep [ Hred [ Hval' Hsub' ] ] ] ] ].
+  apply IHHsub in Hval' ; clear IHHsub ; auto.
+  destruct Hval' as [ x' [ g' [ Hred [ Hval' Hsub' ] ] ] ].
+  destruct (classic (sub X L x' g' g)) as [ His_sub | Hno_sub ].
+  exists x' ; exists (box g) ; repeat split ; auto.
+  apply zero_box_incl with g' ; auto.
+  intros x'' Htrans ; apply Hval.
+  apply trans_closed with x' e ; auto.
+  apply zero_impl_step in Hred ; auto.
+  apply sub_box ; apply sub_trans with g' ; auto.
   exists x' ; exists (conj (box g) g') ; repeat split ; auto.
-  apply red_box ; auto.
+  apply zero_box_excl ; auto.
   intros x'' Htrans ; apply Hval.
   apply trans_closed with x' e ; auto.
-  apply sub_and_right ; auto.
+  apply zero_impl_step in Hred ; auto.
+  apply sub_conj_right ; auto.
 Qed.
 
-Lemma wf_next : forall (f f' : F) (X : Set) (L : X -> P -> Prop)
-  (step : X -> E -> X -> Prop) (x x' : X) (e : E), wf f -> U e ->
-  val (klts X L step x) f -> step x e x' -> red X L x f e f' ->
-  val (klts X L step x') f'.
-Proof.
-  intros f f' X L step x x' e Hwf HU Hval Hstep Hred ;
-    induction Hred ; solve [ simpl ; auto ] || idtac.
-  simpl in * ; destruct Hwf ; destruct Hval ; split ; auto.
-  simpl in Hval ; destruct Hval ; contradiction || auto.
-  simpl in Hwf ; destruct Hwf ; contradiction.
-  simpl in * ; split ; try tauto.
-  intros x'' Htrans ; apply Hval.
-  apply trans_closed with x' e ; auto.
-  apply IHHred ; auto.
-  apply Hval ; apply trans_refl.
-Qed.
-
-Lemma wf_red : forall (f f' : F) (X : Set) (L : X -> P -> Prop)
-  (x : X) (e : E), red X L x f e f' -> wf f -> wf f'.
-Proof.
-  intros f f' X L x e Hred Hwf ; induction Hred ;
-    solve [ simpl in * ; tauto ] || idtac.
-Qed.
-
-Lemma strong_ind : forall (Q : nat -> Prop), Q 0 ->
-  (forall (n : nat), (forall (m : nat), m < n -> Q m) ->
-    Q n) -> forall (n : nat), Q n.
-Proof.
-  intros Q Hzero Hind n ; apply Hind.
-  induction n ; intros m Hless ; inversion Hless.
-  apply Hind ; auto.
-  apply IHn ; auto.
-Qed.
-
-Lemma rel_ex : forall (n : nat) (X : Set) (L : X -> P -> Prop)
-  (step : X -> E -> X -> Prop) (x x' : X) (f f' : F) (e : E),
-  step x e x' -> red X L x f e f' -> (forall (n' : nat) (x'' : X) (f'' : F),
-  n' < n -> trans (X * F) (unctrl (X * F) (rel n' X L step)) (x', f') (x'', f'') ->
-  syn X L (rel n' X L step) (x'', f'') f'') -> rel n X L step (x, f) e (x', f').
-Proof.
-  intro n ; induction n ; 
-    intros X L step x x' f f' e Hstep Hred Hunctrl_syn ;
-    simpl ; split ; auto.
-  right ; intros xf'' Htrans ; destruct xf'' as [ x'' f'' ].
-  apply Hunctrl_syn ; auto.
-Qed.
-
-Lemma trans_pres_wf : forall (X : Set) (L : X -> P -> Prop)
-  (step : X * F -> E -> X * F -> Prop) (x x' : X) (f f' : F),
-  (forall (y y' : X) (g g' : F) (e : E), step (y, g) e (y', g') ->
-    red X L y g e g') -> trans (X * F) step (x, f) (x', f') -> wf f -> wf f'.
-Proof.
-  intros X L step x x' f f' Himpl Htrans Hwf.
-  assert (exists xf : X * F, xf = (x, f)) as Hex by eauto.
-  assert (exists xf' : X * F, xf' = (x', f')) as Hex' by eauto.
-  destruct Hex as [ xf Heq ] ; rewrite <- Heq in *.
-  destruct Hex' as [ xf' Heq' ] ; rewrite <- Heq' in *.
-  revert Heq Heq' Hwf ; revert x f x' f'.
-  induction Htrans ; intros z f z' f' Heq Heq' Hwf.
-  rewrite Heq' in * ; inversion Heq ; auto.
-  destruct x as [ x g ] ; destruct y as [ y g' ].
-  assert ((y, g') = (y, g')) as H' by auto.
-  apply IHHtrans with (x'0 := z') (f' := f') in H' ; auto.
-  apply Himpl in H ; auto.
-  inversion Heq ; replace f with g in * by auto.
-  apply wf_red in H ; auto.
-Qed.
-
-Lemma trans_rtl_ex : forall (n : nat) (X' X : Set) 
-  (L' : X' -> P -> Prop) (L : X -> P -> Prop) 
-  (step' : X' -> E -> X' -> Prop)(step : X -> E -> X -> Prop) 
-  (x' : X') (x y : X) (f f' : F), val (klts X' L' step' x') f ->  wf f -> 
+(* 
+ * This lemma relates partial bisimulation and validity
+ * over a number of uncontrollable steps 
+ *)
+Lemma trans_unctrl_rel : forall (n : nat) (f f' : F) (X X' : Set) (L' : X' -> P -> Prop)
+  (L : X -> P -> Prop) (step' : X' -> E -> X' -> Prop) (step : X -> E -> X -> Prop) 
+  (x' : X') (x y : X), pbis (klts X' L' step' x') (klts X L step x) -> 
   trans (X * F) (unctrl (X * F) (rel n X L step)) (x, f) (y, f') ->
-  pbis (klts X' L' step' x') (klts X L step x) ->
-  exists y' : X', trans X' step' x' y' /\ val (klts X' L' step' y') f' /\ 
-  pbis (klts X' L' step' y') (klts X L step y).
+  fval (klts X' L' step' x') f -> wf f -> exists y' : X',
+  pbis (klts X' L' step' y') (klts X L step y) /\
+  fval (klts X' L' step' y') f' /\ wf f'.
 Proof.
-  intros n X' X L' L step' step x' x y f f' Hval Hwf Htrans Hpbis.
+  intros n f f' X X' L' L step' step x' x y Hpbis Htrans Hval Hwf.
   assert (exists xf : X * F, xf = (x, f)) as Hex by eauto.
   assert (exists yf' : X * F, yf' = (y, f')) as Hex' by eauto.
   destruct Hex as [ xf Heq ] ; rewrite <- Heq in *.
   destruct Hex' as [ yf' Heq' ] ; rewrite <- Heq' in *.
-  revert Hval Hpbis Hwf Heq Heq' ; revert x f y f' x'.
-  induction Htrans ; intros z f z' f' w Hval Hpbis Hwf Heq Heq'.
-  rewrite Heq' in * ; inversion Heq.
-  replace z with z' in * by auto.
-  replace f' with f in * by auto.
-  exists w ; repeat split ; apply trans_refl || auto.
+  revert Heq Heq' Hpbis Hval Hwf ; revert x f y f' x'.
+  induction Htrans ; intros z f z' f' x'' Heq Heq' Hpbis Hval Hwf.
+  rewrite Heq in * ; inversion Heq'.
+  replace z with z' in * by auto ; replace f with f' in * by auto.
+  exists x'' ; repeat split ; auto.
   unfold unctrl in H ; destruct H as [ Hrel HU ].
-  rewrite Heq in * ; destruct y as [ y g ].
-  apply rel_impl_step_red in Hrel.
-  destruct Hrel as [ Hstep Hred ].
-  assert (pbis (klts X' L' step' w) (klts X L step z)) as Hpbis' by auto.
+  rewrite Heq in * ; destruct y as [ w g ].
+  assert (step z e w) as Hstep.
+  apply rel_impl_zero in Hrel ; apply zero_impl_step in Hrel ; auto.
+  assert (zero X L step (z, f) e (w, g)) as Hred.
+  apply rel_impl_zero in Hrel ; auto.
+  assert (pbis (klts X' L' step' x'') (klts X L step z)) as Hpbis' by auto.
   destruct Hpbis as [ R [ HinR HrelR ] ].
   apply HrelR in HinR ; apply HinR in Hstep ; auto.
-  destruct Hstep as [ w' [ Hstep' HR' ] ].
-  assert (val (klts X' L' step' w') g) as Hval'.
-  apply wf_next with (f := f) (x := w) (e := e) ; auto.
-  apply pbis_red with (f := f) (e := e) (f' := g) in Hpbis' ; tauto.
-  apply IHHtrans with (y0 := z') (x := y) (f' := f') in Hval' ; auto.
-  destruct Hval' as [ w'' [ Htrans' [ Hval' HR'' ] ] ].
-  exists w'' ; repeat split ; auto.
-  apply trans_closed with w' e ; auto.
-  apply wf_red in Hred ; auto.
+  destruct Hstep as [ w' [ Hstep' HR ] ].
+  apply wf_next with (f' := g) (x' := w') (e := e) in Hval ; auto.
+  apply IHHtrans with (x := w) (f := g) (x'0 := w') ; auto.
   exists R ; split ; auto.
-  apply wf_red in Hred ; auto.
+  apply wf_zero in Hred ; auto.
+  apply pbis_zero with (X := X) (X' := X') (L := L) (L' := L')
+    (step := step) (step' := step') (x' := x'') (y' := w')
+    (x := z) (y := w) (f := f) (e := e) (f' := g) in Hpbis' ; try tauto.
+  exists R ; split ; auto.
+  apply rel_impl_zero in Hrel ; apply zero_impl_step in Hrel ; auto.
 Qed.
 
-Lemma pbis_impl_syn : forall (n : nat) (f g : F) (X : Set) (L : X -> P -> Prop)
-  (step : X -> E -> X -> Prop) (x : X) (k' : K), sub X L x f g -> wf g ->
-  pbis k' (klts X L step x) -> val k' g -> syn X L (rel n X L step) (x, g) f.
+(*
+ * This is the hardest lemma of the entire proof. It
+ * details how a partial bisimulant, which satisifies a
+ * formula g, implies synthesizability for f, if f is a
+ * sub-formula of g. Note how this requires the well-formedness
+ * test: it is absolutely required that <e>f formulas are
+ * restricted in such a way that e is controllable
+ *)
+Lemma pbis_impl_syn : forall (n : nat) (f g : F) (X X' : Set) (L' : X' -> P -> Prop)
+  (L : X -> P -> Prop) (step' : X' -> E -> X' -> Prop) (step : X -> E -> X -> Prop) 
+  (x' : X') (x : X), pbis (klts X' L' step' x') (klts X L step x) ->
+  wf g -> fval (klts X' L' step' x') g -> sub X L x f g -> syn X L (rel n X L step) (x, g) f.
 Proof.
-  intro n ; induction n using strong_ind ; intro f ; induction f ;
-    intros g X L step x k' Hsub Hwf Hpbis Hval ;
-    solve [ apply syn_all ] || solve [ apply sub_and in Hsub ; 
-    destruct Hsub as [ Hf1 Hf2 ] ; apply syn_and ; 
-    [ apply IHf1 with k' | apply IHf2 with k' ] ; auto ] || auto.
-  destruct k' as [ X' L' step' x' ].
-  apply sub_val with (f := basic b) in Hval ; auto.
-  simpl in Hval ; apply syn_basic.
-  apply pbis_bval with (b := b) in Hpbis ; tauto.
+  intro n ; induction n ; intro f ; induction f ;
+    intros g X X' L' L step' step x' x Hpbis Hwf Hval Hsub.
+  apply syn_basic ; apply sub_val with (f := basic b) in Hval.
+  simpl in Hval ; apply pbis_bval with (b := b) in Hpbis ; tauto.
   apply pbis_sub with (f := basic b) (g := g) in Hpbis ; tauto.
+  apply sub_conj in Hsub ; destruct Hsub ; apply syn_conj ; auto.
+  apply IHf1 with X' L' step' x' ; auto.
+  apply IHf2 with X' L' step' x' ; auto.
   destruct (classic (bval X L x b)) as [ Hbval | Hnot_bval ].
-  apply syn_or_left ; auto.
-  apply sub_not_or in Hsub ; auto.
-  apply syn_or_right ; apply IHf with k' ; auto.
-  destruct k' as [ X' L' step' x' ].
-  apply ex_next with (f := f) (e := e) in Hval ; auto.
-  destruct Hval as [ y' [ g' [ Hstep' [ Hred [ Hval Hsub' ] ] ] ] ].
-  assert (red X L x g e g') as Hred'.
-  apply pbis_red with (f := g) (e := e) (f' := g') in Hpbis ; tauto.
+  apply syn_disj_left ; auto.
+  apply sub_disj_not in Hsub ; auto.
+  apply syn_disj_right.
+  apply IHf with X' L' step' x' ; auto.
+  apply syn_all.
+  assert (pbis (klts X' L' step' x') (klts X L step x)) as Hpbis' by auto.
+  apply ex_next with (e := e) (f := f) in Hval ; auto.
+  destruct Hval as [ y' [ g' [ Hred [ Hval Hsub' ] ] ] ].
   destruct Hpbis as [ R [ HinR HrelR ] ].
+  assert (step' x' e y') as Hstep'.
+  apply zero_impl_step in Hred ; auto.
   apply HrelR in HinR ; apply HinR in Hstep'.
   destruct Hstep' as [ y [ Hstep HR ] ].
-  apply syn_ex with y g' ; auto.
-  simpl ; split ; auto.
-  assert (pbis (klts X' L' step' y') (klts X L step y)) as Hpbis.
+  apply syn_ex with y g' ; simpl ; auto.
+  apply pbis_zero with (X := X) (X' := X') (L := L) (L' := L')
+    (step' := step') (step := step) (x' := x') (x := x)
+    (y' := y') (y := y) (f := g) (e := e) (f' := g') in Hpbis' ; try tauto.
+  apply zero_impl_step in Hred ; auto.
   exists R ; split ; auto.
-  apply pbis_sub with (f := f) (g := g') in Hpbis ; tauto.
-  apply IHf with (k' := klts X' L' step' y') ; auto.
-  assert (pbis (klts X' L' step' y') (klts X L step y)) as Hpbis.
+  assert (pbis (klts X' L' step' y') (klts X L step y)) as Hpbis''.
   exists R ; split ; auto.
-  apply pbis_sub with (f := f) (g := g') in Hpbis ; tauto.
-  apply wf_red in Hred ; auto.
+  apply pbis_sub with (f := f) (g := g') in Hpbis'' ; tauto.
+  assert (pbis (klts X' L' step' y') (klts X L step y)) as Hpbis''.
   exists R ; split ; auto.
+  apply IHf with (g := g') in Hpbis'' ; simpl in * ; auto.  
+  apply wf_zero in Hred ; auto.
+  apply pbis_sub with (f := f) (g := g') in Hpbis'' ; tauto.
   apply pbis_sub with (f := ex e f) (g := g) in Hpbis ; tauto.
-  apply sub_box_impl with (f := f) in Hsub ; auto.
-  apply syn_box ; apply IHf with k' ; auto.
-  destruct k' as [ X' L' step' x' ].
-  assert (val (klts X' L' step' x') (diam b)) as Hval'.
+  apply syn_box ; apply IHf with X' L' step' x' ; auto.
+  apply sub_trans_box with step x g 0 ; apply trans_refl || auto ; auto.
   apply sub_val with (f := diam b) in Hval ; auto.
-  apply pbis_sub with (f := diam b) (g := g) in Hpbis ; tauto.
-  simpl in Hval' ; destruct Hval' as [ y' [ Htrans Hvalb ] ].
-  clear Hsub ; revert Hwf Hpbis Hval.
-  revert g x ; induction Htrans ; intros g z Hwf Hpbis Hval.
-  apply syn_diam with z g ; apply trans_refl || auto ; auto.
+  simpl in Hval ; destruct Hval as [ y' [ Htrans Hbval ] ].
+  clear Hsub ; revert Hpbis Hwf ; revert x g.
+  induction Htrans ; intros z g Hpbis Hwf.
+  apply syn_diam with z g ; apply trans_refl || auto.
   apply pbis_bval with (b := b) in Hpbis ; tauto.
-  assert (step' x e y) as Hstep' by auto.
-  assert (pbis (klts X' L' step' x) (klts X L step z)) 
-    as Hpbis' by auto.
-  destruct Hpbis as [ R [ HinR HrelR ] ].
-  apply HrelR in HinR ; apply HinR in Hstep'.
-  destruct Hstep' as [ z' [ Hstep HR ] ].
-  assert (step' x e y) as Hstep' by auto.
-  apply val_next with (L := L') (step := step') (f := g)
-    in Hstep' ; auto.
-  destruct Hstep' as [ g' [ Hred Hval' ] ].
-  apply IHHtrans with (x := z') in Hval' ; auto.
-  inversion Hval' ; apply syn_diam with x'0 g'0 ; auto.
+  destruct Hpbis as [ R [ HinR HrelR ] ] ; apply HrelR in HinR.
+  apply HinR in H ; destruct H as [ z' [ Hstep HR ] ].
+  destruct (zero_ex g X L step z z' e) as [ g' Hred ] ; auto.
+  apply IHHtrans with (x := z') (g := g') in Hbval ; auto.
+  inversion Hbval.
+  apply syn_diam with x'0 g'0 ; auto.
   apply trans_closed with (z', g') e ; auto.
-  simpl ; split ; auto.
-  apply pbis_red with (f := g) (e := e) (f' := g') in Hpbis' ; tauto.
-  apply wf_red in Hred ; auto.
   exists R ; split ; auto.
-  destruct k' as [ X' L' step' x' ].
-  assert (val (klts X' L' step' x') (can e)) as Hval'.
-  apply sub_val with (f := can e) in Hval ; auto.
-  apply pbis_sub with (f := can e) (g := g) in Hpbis ; tauto.
-  simpl in Hval' ; destruct Hval' as [ y' Hstep' ].
-  assert (step' x' e y') as H by auto.
-  apply val_next with (step := step') (L := L') (f := g) in H ; auto.
-  destruct H as [ g' [ Hred Hval' ] ].
-  assert (pbis (klts X' L' step' x') (klts X L step x)) as Hpbis' by auto.
-  destruct Hpbis as [ R [ HinR HrelR ] ].
-  apply HrelR in HinR ; apply HinR in Hstep'.
-  destruct Hstep' as [ y [ Hstep HR ] ].
-  apply syn_can with y g' ; simpl ; split ; auto.
-  apply pbis_red with (f := g) (e := e) (f' := g') in Hpbis' ; tauto.
-  destruct k' as [ X' L' step' x' ].
-  assert (val (klts X' L' step' x') dlf) as Hval'.
-  apply sub_val with (f := dlf) in Hval ; auto.
-  apply pbis_sub with (f := dlf) (g := g) in Hpbis ; tauto.
-  simpl in Hval' ; destruct Hval' as [ e [ y' Hstep' ] ].
-  assert (step' x' e y') as H by auto.
-  apply val_next with (step := step') (L := L') (f := g) in H ; auto.
-  destruct H as [ g' [ Hred Hval' ] ].
-  assert (pbis (klts X' L' step' x') (klts X L step x)) as Hpbis' by auto.
-  destruct Hpbis as [ R [ HinR HrelR ] ].
-  apply HrelR in HinR ; apply HinR in Hstep'.
-  destruct Hstep' as [ y [ Hstep HR ] ].
-  apply syn_dlf with y g' e ; simpl ; split ; auto.
-  apply pbis_red with (f := g) (e := e) (f' := g') in Hpbis' ; tauto.
-
-  (* Start inductive case *)
-  destruct k' as [ X' L' step' x' ].
-  apply sub_val with (f := basic b) in Hval ; auto.
-  simpl in Hval ; apply syn_basic.
-  apply pbis_bval with (b := b) in Hpbis ; tauto.
-  apply pbis_sub with (f := basic b) (g := g) in Hpbis ; tauto.
-  destruct (classic (bval X L x b)) as [ Hbval | Hnot_bval ].
-  apply syn_or_left ; auto.
-  apply sub_not_or in Hsub ; auto.
-  apply syn_or_right ; apply IHf with k' ; auto.
-  destruct k' as [ X' L' step' x' ].
-  apply ex_next with (f := f) (e := e) in Hval ; auto.
-  destruct Hval as [ y' [ g' [ Hstep' [ Hred [ Hval Hsub' ] ] ] ] ].
-  assert (red X L x g e g') as Hred'.
-  apply pbis_red with (f := g) (e := e) (f' := g') in Hpbis ; tauto.
-  destruct Hpbis as [ R [ HinR HrelR ] ].
-  apply HrelR in HinR ; apply HinR in Hstep'.
-  destruct Hstep' as [ y [ Hstep HR ] ].
-  apply syn_ex with y g' ; auto.
-  assert (wf g') as Hwf'.
-  apply wf_red in Hred ; auto.
-  apply rel_ex ; auto.
-  intros n' z g'' Hless Htrans_xf.
-  assert (wf g'') as Hwf''.
-  apply trans_pres_wf with (L := L) in Htrans_xf ; auto.
-  intros v v' h h' e' Hunctrl.
-  unfold unctrl in Hunctrl.
-  destruct Hunctrl as [ Hrel _ ].
-  apply rel_impl_step_red in Hrel ; tauto.
-  apply trans_rtl_ex with (X' := X') (L' := L') 
-    (step' := step') (x' := y') in Htrans_xf ; auto.
-  destruct Htrans_xf as [ z' [ Htrans [ Hval' Hpbis ] ] ].
-  apply H with (klts X' L' step' z') ; auto.
-  apply sub_refl.
-  exists R ; split ; auto.
-  assert (pbis (klts X' L' step' y') (klts X L step y)) as Hpbis.
-  exists R ; split ; auto.
-  apply pbis_sub with (f := f) (g := g') in Hpbis ; tauto.
-  apply IHf with (k' := klts X' L' step' y') ; auto.
-  assert (pbis (klts X' L' step' y') (klts X L step y)) as Hpbis.
-  exists R ; split ; auto.
-  apply pbis_sub with (f := f) (g := g') in Hpbis ; tauto.
-  apply wf_red in Hred ; auto.
-  exists R ; split ; auto.
-  apply pbis_sub with (f := ex e f) (g := g) in Hpbis ; tauto.
-  apply sub_box_impl with (f := f) in Hsub ; auto.
-  apply syn_box ; apply IHf with k' ; auto.
-  destruct k' as [ X' L' step' x' ].
-  assert (val (klts X' L' step' x') (diam b)) as Hval'.
-  apply sub_val with (f := diam b) in Hval ; auto.
+  apply wf_zero in Hred ; auto.
   apply pbis_sub with (f := diam b) (g := g) in Hpbis ; tauto.
-  simpl in Hval' ; destruct Hval' as [ y' [ Htrans Hvalb ] ].
-  clear Hsub ; revert Hwf Hpbis Hval.
-  revert g x ; induction Htrans ; intros g z Hwf Hpbis Hval.
-  apply syn_diam with z g ; apply trans_refl || auto ; auto.
-  apply pbis_bval with (b := b) in Hpbis ; tauto.
-  assert (step' x e y) as Hstep' by auto.
-  assert (pbis (klts X' L' step' x) (klts X L step z)) 
-    as Hpbis' by auto.
-  destruct Hpbis as [ R [ HinR HrelR ] ].
-  apply HrelR in HinR ; apply HinR in Hstep'.
-  destruct Hstep' as [ z' [ Hstep HR ] ].
-  assert (step' x e y) as Hstep' by auto.
-  apply val_next with (L := L') (step := step') (f := g)
-    in Hstep' ; auto.
-  destruct Hstep' as [ g' [ Hred Hval' ] ].
-  assert (val (klts X' L' step' y) g') as Hval_bak by auto.
-  apply IHHtrans with (x := z') in Hval' ; auto.
-  inversion Hval' ; apply syn_diam with x'0 g'0 ; auto.
-  apply trans_closed with (z', g') e ; auto.
-  apply rel_ex ; auto.
-  apply pbis_red with (f := g) (e := e) (f' := g') in Hpbis' ; tauto.
-  intros n' x'' g'' Hless Htrans'.
-  assert (wf g'') as Hwf''.
-  apply trans_pres_wf with (L := L) in Htrans' ; auto.
-  intros v v' h h' e' Hunctrl.
-  unfold unctrl in Hunctrl.
-  destruct Hunctrl as [ Hrel _ ].
-  apply rel_impl_step_red in Hrel ; tauto.
-  apply wf_red in Hred ; auto.
-  apply trans_rtl_ex with (X' := X') (L' := L') (step' := step')
-    (x' := y) in Htrans' ; auto.
-  destruct Htrans' as [ y' [ Htrans' [ Hval'' Hpbis ] ] ].
-  apply H with (klts X' L' step' y') ; auto.
-  apply sub_refl.
-  apply wf_red in Hred ; auto.
-  exists R ; split ; auto.
-  apply wf_red in Hred ; auto.
-  exists R ; split ; auto.
-  destruct k' as [ X' L' step' x' ].
-  assert (val (klts X' L' step' x') (can e)) as Hval'.
   apply sub_val with (f := can e) in Hval ; auto.
-  apply pbis_sub with (f := can e) (g := g) in Hpbis ; tauto.
-  simpl in Hval' ; destruct Hval' as [ y' Hstep' ].
-  assert (step' x' e y') as Hstep_bak by auto.
-  apply val_next with (step := step') (L := L') (f := g) in Hstep_bak ; auto.
-  destruct Hstep_bak as [ g' [ Hred Hval' ] ].
-  assert (pbis (klts X' L' step' x') (klts X L step x)) as Hpbis' by auto.
-  destruct Hpbis as [ R [ HinR HrelR ] ].
-  apply HrelR in HinR ; apply HinR in Hstep'.
-  destruct Hstep' as [ y [ Hstep HR ] ].
+  simpl in Hval ; destruct Hval as [ y' Hstep ].
+  destruct Hpbis as [ R [ HinR HrelR ] ] ; apply HrelR in HinR.
+  apply HinR in Hstep ; destruct Hstep as [ y [ Hstep HR ] ].
+  destruct (zero_ex g X L step x y e) as [ g' Hred ] ; auto.
   apply syn_can with y g' ; auto.
-  apply rel_ex ; auto.
-  apply pbis_red with (f := g) (e := e) (f' := g') in Hpbis' ; tauto.
-  intros n' z g'' Hless Htrans.
-  assert (wf g'') as Hwf''.
-  apply trans_pres_wf with (L := L) in Htrans ; auto.
-  intros v v' h h' e' Hunctrl.
-  unfold unctrl in Hunctrl.
-  destruct Hunctrl as [ Hrel _ ].
-  apply rel_impl_step_red in Hrel ; tauto.
-  apply wf_red in Hred ; auto.
-  apply trans_rtl_ex with (X' := X') (L' := L')
-    (step' := step') (x' := y') in Htrans ; auto.
-  destruct Htrans as [ z' [ Htrans [ Hval'' Hpbis'' ] ] ].
-  apply H with (k' := klts X' L' step' z') ; auto.
-  apply sub_refl.
-  apply wf_red in Hred ; auto.
-  exists R ; split ; auto.
-  destruct k' as [ X' L' step' x' ].
-  assert (val (klts X' L' step' x') dlf) as Hval'.
+  apply pbis_sub with (f := can e) (g := g) in Hpbis ; tauto.
   apply sub_val with (f := dlf) in Hval ; auto.
+  simpl in Hval ; destruct Hval as [ e [ y' Hstep ] ].
+  destruct Hpbis as [ R [ HinR HrelR ] ] ; apply HrelR in HinR.
+  apply HinR in Hstep ; destruct Hstep as [ y [ Hstep HR ] ].
+  destruct (zero_ex g X L step x y e) as [ g' Hred ] ; auto.
+  apply syn_dlf with y e g' ; auto.
   apply pbis_sub with (f := dlf) (g := g) in Hpbis ; tauto.
-  simpl in Hval' ; destruct Hval' as [ e [ y' Hstep' ] ].
-  assert (step' x' e y') as Hstep_bak by auto.
-  apply val_next with (step := step') (L := L') (f := g) in Hstep_bak ; auto.
-  destruct Hstep_bak as [ g' [ Hred Hval' ] ].
+
+  (* Inductive case for n *)
+  apply syn_basic ; apply sub_val with (f := basic b) in Hval.
+  simpl in Hval ; apply pbis_bval with (b := b) in Hpbis ; tauto.
+  apply pbis_sub with (f := basic b) (g := g) in Hpbis ; tauto.
+  apply sub_conj in Hsub ; destruct Hsub ; apply syn_conj ; auto.
+  apply IHf1 with X' L' step' x' ; auto.
+  apply IHf2 with X' L' step' x' ; auto.
+  destruct (classic (bval X L x b)) as [ Hbval | Hnot_bval ].
+  apply syn_disj_left ; auto.
+  apply sub_disj_not in Hsub ; auto.
+  apply syn_disj_right.
+  apply IHf with X' L' step' x' ; auto.  
+  apply syn_all.
   assert (pbis (klts X' L' step' x') (klts X L step x)) as Hpbis' by auto.
+  apply ex_next with (e := e) (f := f) in Hval ; auto.
+  destruct Hval as [ y' [ g' [ Hred [ Hval Hsub' ] ] ] ].
   destruct Hpbis as [ R [ HinR HrelR ] ].
+  assert (step' x' e y') as Hstep'.
+  apply zero_impl_step in Hred ; auto.
   apply HrelR in HinR ; apply HinR in Hstep'.
   destruct Hstep' as [ y [ Hstep HR ] ].
-  apply syn_dlf with y g' e ; simpl ; auto.
+  apply syn_ex with y g' ; auto.
+  simpl ; split ; auto.
   apply rel_ex ; auto.
-  apply pbis_red with (f := g) (e := e) (f' := g') in Hpbis' ; tauto.
-  intros n' z g'' Hless Htrans.
-  assert (wf g'') as Hwf''.
-  apply trans_pres_wf with (L := L) in Htrans ; auto.
-  intros v v' h h' e' Hunctrl.
-  unfold unctrl in Hunctrl.
-  destruct Hunctrl as [ Hrel _ ].
-  apply rel_impl_step_red in Hrel ; tauto.
-  apply wf_red in Hred ; auto.
-  apply trans_rtl_ex with (X' := X') (L' := L')
+  intros z g'' Htrans.
+  apply trans_unctrl_rel with (X' := X') (L' := L')
     (step' := step') (x' := y') in Htrans ; auto.
-  destruct Htrans as [ z' [ Htrans [ Hval'' Hpbis'' ] ] ].
-  apply H with (k' := klts X' L' step' z') ; auto.
+  destruct Htrans as [ z' [ Hpbis'' [ Hval' Hwf' ] ] ].
+  apply IHn with (X' := X') (L' := L') (step' := step')
+    (x' := z') ; auto.
   apply sub_refl.
-  apply wf_red in Hred ; auto.
   exists R ; split ; auto.
-Qed.  
-
-Theorem maximality : forall (k' k : K) (f : F) (n : nat),
-  wf f -> pbis k' k -> val k' f -> pbis k' (S k f n).
-Proof.
-  intros k' k f n Hwf Hpbis Hval.
-  destruct k' as [ X' L' step' x' ].
-  destruct k as [ X L step x ].
+  apply wf_zero in Hred ; auto.
+  apply pbis_zero with (X := X) (X' := X') (L := L) (L' := L')
+    (step' := step') (step := step) (x' := x') (x := x)
+    (y' := y') (y := y) (f := g) (e := e) (f' := g') in Hpbis' ; try tauto.
+  apply zero_impl_step in Hred ; auto.
+  exists R ; split ; auto.
+  right ; intros xf'' Htrans.
+  destruct xf'' as [ z g'' ].
+  apply trans_unctrl_rel with (X' := X') (L' := L')
+    (step' := step') (x' := y') in Htrans ; auto.
+  destruct Htrans as [ z' [ Hpbis'' [ Hval' Hwf' ] ] ].
+  apply IHn with (X' := X') (L' := L') (step' := step')
+    (x' := z') ; auto.
+  simpl ; apply sub_refl.
+  exists R ; split ; auto.
+  apply wf_zero in Hred ; auto.
+  assert (pbis (klts X' L' step' y') (klts X L step y)) as Hpbis''.
+  exists R ; split ; auto.
+  apply pbis_sub with (f := f) (g := g') in Hpbis'' ; tauto.
+  apply IHf with (X' := X') (L' := L') (step' := step') (x' := y') ; auto.
+  exists R ; split ; auto.
+  apply wf_zero in Hred ; auto.
+  assert (pbis (klts X' L' step' y') (klts X L step y)) as Hpbis''.
+  exists R ; split ; auto.
+  apply pbis_sub with (f := f) (g := g') in Hpbis'' ; tauto.
+  apply pbis_sub with (f := ex e f) (g := g) in Hpbis' ; tauto.
+  apply syn_box ; apply IHf with (X' := X') (L' := L')
+    (step' := step') (x' := x') ; auto.
+  apply sub_trans_box with (step := step) (x' := x)
+    (g' := g) (n := n) in Hsub ; apply trans_refl || auto.
+  assert (fval (klts X' L' step' x') g) as Hval' by auto.
+  apply sub_val with (f := diam b) in Hval' ; auto.
+  simpl in Hval' ; destruct Hval' as [ y' [ Htrans Hbval ] ].
+  clear Hsub ; revert Hpbis Hwf Hval Hbval ; revert x g.
+  induction Htrans ; intros z g Hpbis Hwf Hval Hbval.
+  apply syn_diam with z g ; apply trans_refl || auto.
+  apply pbis_bval with (b := b) in Hpbis ; tauto.
+  assert (pbis (klts X' L' step' x) (klts X L step z)) as Hpbis' by auto.
+  destruct Hpbis' as [ R [ HinR HrelR ] ] ; apply HrelR in HinR.
+  assert (step' x e y) as Hstep' by auto.
+  apply HinR in H ; destruct H as [ w [ Hstep HR ] ].
+  apply val_next with (x' := y) (e := e) in Hval ; auto.
+  destruct Hval as [ g' [ Hred Hval ] ].
+  assert (pbis (klts X' L' step' y) (klts X L step w)) as Hpbis'.
+  exists R ; split ; auto.
+  apply IHHtrans with (g := g') in Hpbis' ; auto.
+  inversion Hpbis'.
+  apply syn_diam with x'0 g'0 ; auto.
+  apply trans_closed with (w, g') e ; auto.
+  simpl ; split ; auto.
+  apply rel_ex ; auto.
+  intros w' g'' Htrans'.
+  apply trans_unctrl_rel with (X' := X') (L' := L')
+    (step' := step') (x' := y) in Htrans' ; auto.
+  destruct Htrans' as [ y' [ Hpbis'' [ Hval' Hwf' ] ] ].
+  apply IHn with (X' := X') (L' := L') (step' := step')
+    (x' := y') ; auto.
+  apply sub_refl.
+  exists R ; split ; auto.
+  apply wf_zero in Hred ; auto.
+  apply pbis_zero with (X := X) (X' := X') (L := L) (L' := L')
+    (step' := step') (step := step) (x' := x) (x := z)
+    (y' := y) (y := w) (f := g) (e := e) (f' := g') in Hpbis ; try tauto.
+  exists R ; split ; auto.
+  right ; intros xf'' Htrans' ; destruct xf'' as [ w' g'' ].
+  apply trans_unctrl_rel with (X' := X') (L' := L')
+    (step' := step') (x' := y) in Htrans' ; auto.
+  destruct Htrans' as [ y' [ Hpbis'' [ Hval' Hwf' ] ] ].
+  apply IHn with (X' := X') (L' := L') (step' := step')
+    (x' := y') ; auto.
+  apply sub_refl.
+  exists R ; split ; auto.
+  apply wf_zero in Hred ; auto.
+  apply wf_zero in Hred ; auto.
+  apply pbis_sub with (f := diam b) (g := g) in Hpbis ; tauto.
+  assert (fval (klts X' L' step' x') g) as Hval' by auto.
+  apply sub_val with (f := can e) in Hval' ; auto.
+  simpl in Hval' ; destruct Hval' as [ y' Hstep ].
+  assert (step' x' e y') as Hstep' by auto.
+  apply val_next with (f := g) (X := X') (L := L')
+    (step := step') (x := x') (e := e) (x' := y') in Hstep ; auto.
+  destruct Hstep as [ g' [ Hred Hval' ] ].
+  assert (pbis (klts X' L' step' x') (klts X L step x)) as Hpbis' by auto.
   destruct Hpbis as [ R [ HinR HrelR ] ].
-  exists (fun y' yg => R y' (fst yg) /\ wf (snd yg) /\
-    val (klts X' L' step' y') (snd yg)) ; split ; auto.
+  apply HrelR in HinR ; apply HinR in Hstep' ; auto.
+  destruct Hstep' as [ y [ Hstep HR ] ].
+  apply syn_can with (x' := y) (g' := g') ; auto.
+  simpl ; split ; auto.
+  apply rel_ex ; auto.
+  intros z g'' Htrans.
+  apply trans_unctrl_rel with (X' := X') (L' := L')
+    (step' := step') (x' := y') in Htrans ; auto.
+  destruct Htrans as [ z' [ Hpbis'' [ Hval'' Hwf' ] ] ].
+  apply IHn with (X' := X') (L' := L') (step' := step')
+    (x' := z') ; apply sub_refl || auto.
+  exists R ; split ; auto.
+  apply wf_zero in Hred ; auto.
+  apply pbis_zero with (X := X) (X' := X') (L := L) (L' := L')
+    (step' := step') (step := step) (x' := x') (x := x)
+    (y' := y') (y := y) (f := g) (e := e) (f' := g') in Hpbis' ; try tauto.
+  apply zero_impl_step in Hred ; auto.
+  exists R ; split ; auto.
+  right ; intros xf'' Htrans ; destruct xf'' as [ z g'' ].
+  apply trans_unctrl_rel with (X' := X') (L' := L')
+    (step' := step') (x' := y') in Htrans ; auto.
+  destruct Htrans as [ z' [ Hpbis'' [ Hval'' Hwf' ] ] ].
+  apply IHn with (X' := X') (L' := L') (step' := step')
+    (x' := z') ; apply sub_refl || auto.
+  exists R ; split ; auto.
+  apply wf_zero in Hred ; auto.
+  apply pbis_sub with (f := can e) (g := g) in Hpbis ; tauto.
+  assert (fval (klts X' L' step' x') g) as Hval' by auto.
+  apply sub_val with (f := dlf) in Hval' ; auto.
+  simpl in Hval' ; destruct Hval' as [ e [ y' Hstep ] ].
+  assert (step' x' e y') as Hstep' by auto.
+  apply val_next with (f := g) (X := X') (L := L')
+    (step := step') (x := x') (e := e) (x' := y') in Hstep ; auto.
+  destruct Hstep as [ g' [ Hred Hval' ] ].
+  assert (pbis (klts X' L' step' x') (klts X L step x)) as Hpbis' by auto.
+  destruct Hpbis as [ R [ HinR HrelR ] ].
+  apply HrelR in HinR ; apply HinR in Hstep' ; auto.
+  destruct Hstep' as [ y [ Hstep HR ] ].
+  apply syn_dlf with (e := e) (x' := y) (g' := g') ; auto.
+  simpl ; split ; auto.
+  apply rel_ex ; auto.
+  intros z g'' Htrans.
+  apply trans_unctrl_rel with (X' := X') (L' := L')
+    (step' := step') (x' := y') in Htrans ; auto.
+  destruct Htrans as [ z' [ Hpbis'' [ Hval'' Hwf' ] ] ].
+  apply IHn with (X' := X') (L' := L') (step' := step')
+    (x' := z') ; apply sub_refl || auto.
+  exists R ; split ; auto.
+  apply wf_zero in Hred ; auto.
+  apply pbis_zero with (X := X) (X' := X') (L := L) (L' := L')
+    (step' := step') (step := step) (x' := x') (x := x)
+    (y' := y') (y := y) (f := g) (e := e) (f' := g') in Hpbis' ; try tauto.
+  apply zero_impl_step in Hred ; auto.
+  exists R ; split ; auto.
+  right ; intros xf'' Htrans ; destruct xf'' as [ z g'' ].
+  apply trans_unctrl_rel with (X' := X') (L' := L')
+    (step' := step') (x' := y') in Htrans ; auto.
+  destruct Htrans as [ z' [ Hpbis'' [ Hval'' Hwf' ] ] ].
+  apply IHn with (X' := X') (L' := L') (step' := step')
+    (x' := z') ; apply sub_refl || auto.
+  exists R ; split ; auto.
+  apply wf_zero in Hred ; auto.
+  apply pbis_sub with (f := dlf) (g := g) in Hpbis ; tauto.
+Qed.
+
+(* Prove that the synthesis result is maximal *)
+Theorem maximality : forall (k' k : K) (f : F) (n : nat),
+  wf f -> pbis k' k -> fval k' f -> pbis k' (S k f n).
+Proof.
+  intros k' k f n Hwf Hpbis Hval ; destruct k' as [ X' L' step' x' ].
+  destruct k as [ X L step x ] ; destruct Hpbis as [ R [ HinR HrelR ] ].
+  exists (fun y' yg => R y' (fst yg) /\ wf (snd yg) /\ 
+    fval (klts X' L' step' y') (snd yg)) ; split ; auto.
   intros y' yg H ; destruct H as [ HR [ Hwf' Hval' ] ].
-  destruct yg as [ y g ] ; simpl in *.
-  assert (R y' y) as HR_bak by auto.
+  destruct yg as [ y g ] ; simpl in HR ; simpl in Hval' ; simpl.
+  assert (pbis (klts X' L' step' y') (klts X L step y)) as Hpbis.
+  exists R ; split ; auto.
   apply HrelR in HR ; split ; [ tauto | split ].
-  intros e z' Hstep' ; assert (step' y' e z') as H by auto.
-  apply val_next with (f := g) (X := X') (L := L') (step := step')
-    (x := y') (e := e) (x' := z') in H ; auto.
-  destruct H as [ g' [ Hred Hval'' ] ].
-  assert (step' y' e z') as Hstep_bak by auto.
+  intros e z' Hstep'.
+  assert (exists f' : F, zero X' L' step' (y', g) e (z', f') /\ 
+    fval (klts X' L' step' z') f') as Hex.
+  apply val_next ; auto.
+  destruct Hex as [ g' [ Hred Hval'' ] ].
   apply HR in Hstep' ; destruct Hstep' as [ z [ Hstep HR' ] ].
   exists (z, g') ; repeat split ; auto.
   apply rel_ex ; auto.
-  assert (pbis (klts X' L' step' y') (klts X L step y)) as Hpbis.
-  exists R ; split ; auto.
-  apply pbis_red with (f := g) (e := e) (f' := g') in Hpbis ; tauto.
-  intros n' x'' g'' Hless Htrans.
+  intros w g'' Htrans.
   assert (wf g') as Hwf''.
-  apply wf_red in Hred ; auto.
-  assert (exists z'' : X', trans X' step' z' z'' /\
-    val (klts X' L' step' z'') g'' /\ R z'' x'') as H'.
-  clear HinR Hstep Hred Hless Hwf Hstep_bak HR_bak HR Hval' Hval Hwf'.
-  assert (exists zg : X * F, zg = (z, g')) as Hex by eauto.
-  assert (exists xg : X * F, xg = (x'', g'')) as Hex' by eauto.
-  destruct Hex as [ yg Heq ] ; rewrite <- Heq in *.
-  destruct Hex' as [ zg Heq' ] ; rewrite <- Heq' in *.
-  revert Hval'' HR' Hwf'' Heq Heq' ; revert z g' x'' g'' z'.
-  induction Htrans ; intros w g' z g'' z' Hval HR Hwf Heq Heq'.
-  rewrite Heq' in * ; inversion Heq.
-  replace z with w in * by auto.
-  replace g'' with g' in * by auto.
-  exists z' ; repeat split ; apply trans_refl || auto.
-  unfold unctrl in H ; destruct H as [ Hrel HU ].
-  rewrite Heq in * ; destruct y0 as [ v h ].
-  apply rel_impl_step_red in Hrel.
-  destruct Hrel as [ Hstep Hred ].
-  assert (R z' w) as HR_bak by auto.
+  apply wf_zero in Hred ; auto.
+  assert (exists w' : X', trans X' step' z' w' /\ wf g'' /\
+    R w' w /\ fval (klts X' L' step' w') g'') as H.
+  clear HinR HR Hstep Hred Hval' Hwf Hval.
+  assert (exists zg' : X * F, zg' = (z, g')) as Heq by eauto.
+  assert (exists wg'' : X * F, wg'' = (w, g'')) as Heq' by eauto.
+  destruct Heq as [ zg' Heq ] ; rewrite <- Heq in *.
+  destruct Heq' as [ wg'' Heq' ] ; rewrite <- Heq' in *.
+  revert Heq Heq' HR' Hval'' Hwf'' ; revert z g' w g'' z'.
+  induction Htrans ; intros z g' w g'' z' Heq Heq' HR Hval Hwf.
+  rewrite Heq in * ; inversion Heq'.
+  replace g' with g'' in * ; auto.
+  replace z with w in * ; auto.
+  exists z' ; repeat split ; apply trans_refl || auto ; auto.
+  rewrite Heq in * ; unfold unctrl in H.
+  destruct H as [ Hrel HU ] ; destruct y0 as [ v h ].
+  assert (step z e0 v) as Hstep.
+  apply rel_impl_zero in Hrel ; apply zero_impl_step in Hrel ; auto.
+  assert (zero X L step (z, g') e0 (v, h)) as Hred.
+  apply rel_impl_zero in Hrel ; auto.
+  assert (pbis (klts X' L' step' z') (klts X L step z)) as Hpbis'.
+  exists R ; split ; auto.
   apply HrelR in HR ; apply HR in Hstep ; auto.
-  destruct Hstep as [ v' [ Hstep' HR' ] ].
-  assert (val (klts X' L' step' v') h) as Hval'.
-  apply wf_next with (f := g') (x := z') (e := e0) ; auto.
-  assert (pbis (klts X' L' step' z') (klts X L step w)) as Hpbis.
+  destruct Hstep as [ v' [ Hstep' HR' ] ] ; clear HR.
+  assert (fval (klts X' L' step' v') h) as Hval'.
+  apply wf_next with g' z' e0 ; auto.
+  apply pbis_zero with (X := X) (X' := X') (L := L) (L' := L')
+    (step' := step') (step := step) (x' := z') (x := z)
+    (y' := v') (y := v) (f := g') (e := e0) (f' := h) in Hpbis' ; try tauto.
   exists R ; split ; auto.
-  apply pbis_red with (f := g') (e := e0) (f' := h) in Hpbis ; tauto.
-  apply IHHtrans with (z' := v') (z := v) (x'' := z) (g'' := g'') in Hval' ; auto.
-  destruct Hval' as [ z'' [ Htrans' [ Hval' HR'' ] ] ].
-  exists z'' ; repeat split ; auto.
+  apply zero_impl_step in Hred ; auto.
+  apply IHHtrans with (z := v) (w := w) (g'' := g'') 
+    in Hval' ; auto.
+  destruct Hval' as [ w' [ Htrans' [ Hwf'' [ HR'' Hval' ] ] ] ].
+  exists w' ; repeat split ; auto.
   apply trans_closed with v' e0 ; auto.
-  apply wf_red in Hred ; auto.
-  destruct H' as [ w' [ Htrans' [ Hval''' HR'' ] ] ].
-  apply pbis_impl_syn with (k' := klts X' L' step' w') ; auto.
+  apply wf_zero in Hred ; auto.
+  destruct H as [ w' [ _ [ Hwf''' [ HR'' Hval''' ] ] ] ].
+  apply pbis_impl_syn with (X' := X') (L' := L')
+    (step' := step') (x' := w') ; auto.
+  exists R ; split ; auto.
   apply sub_refl.
-  apply trans_pres_wf with (L := L) in Htrans ; auto.
-  intros t t' h h' e' Hrel.
-  unfold unctrl in Hrel.
-  destruct Hrel as [ Hrel _ ].
-  apply rel_impl_step_red in Hrel ; tauto.
+  apply pbis_zero with (X := X) (X' := X') (L := L) (L' := L')
+    (step' := step') (step := step) (x' := y') (x := y)
+    (y' := z') (y := z) (f := g) (e := e) (f' := g') in Hpbis ; try tauto.
+  apply zero_impl_step in Hred ; auto.
   exists R ; split ; auto.
-  simpl ; apply wf_red in Hred ; auto.
-  assert (pbis (klts X' L' step' y') (klts X L step y)) as Hpbis.
-  exists R ; split ; auto.
+  simpl in * ; apply wf_zero in Hred ; auto.
   intros e z HU Hrel ; destruct z as [ z g' ].
-  apply rel_impl_step_red in Hrel.
-  destruct Hrel as [ Hstep Hred ].
-  assert (pbis (klts X' L' step' y') (klts X L step y)) as Hpbis'.
-  exists R ; split ; auto.
-  apply HrelR in HR_bak ; apply HR_bak in Hstep ; auto.
-  destruct Hstep as [ z' [ Hstep' HR' ] ].
+  assert (zero X L step (y, g) e (z, g')) as Hred.
+  apply rel_impl_zero in Hrel ; auto.
+  apply zero_impl_step in Hred.
+  apply HR in Hred ; auto.
+  destruct Hred as [ z' [ Hstep' HR' ] ].
   exists z' ; repeat split ; auto.
-  simpl ; apply wf_red in Hred ; auto.
-  simpl ; apply wf_next with (f := g) (x := y') (e := e) ; auto.
-  apply pbis_red with (f := g) (e := e) (f' := g') in Hpbis' ; tauto.
+  apply rel_impl_zero in Hrel.
+  apply wf_zero in Hrel ; simpl in * ; auto.
+  simpl in * ; apply wf_next with g y' e ; auto.
+  apply pbis_zero with (X := X) (X' := X') (L := L) (L' := L')
+    (step' := step') (step := step) (x' := y') (x := y)
+    (y' := z') (y := z) (f := g) (e := e) (f' := g') in Hpbis ; try tauto.
+  apply rel_impl_zero in Hrel ; tauto.
+  exists R ; split ; auto.
+  apply rel_impl_zero in Hrel ; apply zero_impl_step in Hrel ; auto.
 Qed.
